push consensus State aside, add btExtend properties

Structures/BlockTree.v
@@ -10,6 +10,8 @@ Unset Strict Implicit.
 Unset Printing Implicit Defensive.
 
 (* A formalization of a block forests *)
+(*Some bits and pieces (btExtend relation properties) taken from *)
+(*https://github.com/certichain/toychain *)
 
 (************************************************************)
 (******************* <parameters> ***************************)
@@ -92,797 +94,633 @@ Proof. by move=>Vh h c; rewrite findF;case: ifP=>//_ /Vh. Qed.
 Lemma validH_undef : validH um_undef.
 Proof. by rewrite/validH=>h b; rewrite find_undef. Qed.
 
-(************************************************************)
-(** Consensus State                                        **)
-(************************************************************)
-
-Record ConsensusState := mkConsensusState {
-  last_vote_round: nat;
-  preferred_block_round: nat;
-}.
-
-Definition consensusstate2nats (cs: ConsensusState) :=
-  let: mkConsensusState lvr pvr := cs in (lvr, pvr).
-
-Definition nats2consensusstate (nats: nat * nat) :=
-  let: (lvr, pbr) := nats in mkConsensusState lvr pbr.
-
-Lemma can_cs_nats: ssrfun.cancel consensusstate2nats nats2consensusstate.
-Proof. by move => []. Qed.
-
-Definition cs_eqMixin := CanEqMixin can_cs_nats.
-Canonical cs_eqType := EqType _ cs_eqMixin.
-
-Definition genesis_state := mkConsensusState genesis_round genesis_round.
-
-Implicit Type state: ConsensusState.
-
-Definition update state (qc: QC) :=
-  let: round := (block_round (qc_vote_data qc)) in
-  if (round > preferred_block_round state) then
-    mkConsensusState (last_vote_round state) (round)
-  else
-    state.
-
-Lemma update_eq_lvr state qc :
-  last_vote_round (update state qc) = last_vote_round state.
-Proof.
-rewrite /update.
-by case (block_round (qc_vote_data qc) > preferred_block_round state).
-Qed.
-
-Lemma update_pbr_geq state qc :
-  preferred_block_round state <= preferred_block_round (update state qc).
-Proof.
-rewrite /update.
-case H: (block_round (qc_vote_data qc) > preferred_block_round state) => //.
-by move/ltnW: H => ->.
-Qed.
-
-Lemma update_qc_gt state qc :
-  block_round (qc_vote_data qc) <= preferred_block_round (update state qc).
-Proof.
-rewrite /update; case H: (preferred_block_round state < (block_round (qc_vote_data qc))) => //.
-by rewrite leqNgt H.
-Qed.
-
-Lemma update_pbr_P state qc:
-  reflect (preferred_block_round (update state qc) = block_round (qc_vote_data qc))
-          (preferred_block_round state <= block_round (qc_vote_data qc)).
-Proof.
-apply: (iffP idP); rewrite /update;
-case H: (block_round (qc_vote_data qc) > preferred_block_round state);
-rewrite leq_eqVlt H ?orbF ?orbT //; move/eqP=> //.
-Qed.
-
-Lemma update_maxn state qc:
-  update state qc =
-  mkConsensusState (last_vote_round state)
-                   (maxn (preferred_block_round state) (block_round (qc_vote_data qc))).
-Proof.
-rewrite /update /maxn; case: ((preferred_block_round state) < (block_round (qc_vote_data qc))) => //=.
-by case state.
-Qed.
-
-(************************************************************)
-(** Voting after update with the QC                        **)
-(************************************************************)
-
-Definition votable state b :=
-  let: (rd, lvr, pbr) :=
-     ((round b),
-     (last_vote_round state),
-     (preferred_block_round state)) in [&& rd > lvr & rd >= pbr].
-
-Lemma votable_updateP state b:
-  reflect (votable (update state (qc_of b)) b)
-  (votable state b && (round b >= block_round (qc_vote_data (qc_of b)))).
-Proof.
-  apply: (iffP andP); rewrite /votable update_eq_lvr.
-- rewrite /update; case (preferred_block_round state < block_round (qc_vote_data (qc_of b)));
-  by move=> [H1 H2]; move/andP: H1=> [-> H1] //; rewrite ltnW //.
-- move/andP => [->] //= H.
-  apply/andP; rewrite (leq_trans (update_pbr_geq _ _) H) //=.
-  by apply: (leq_trans (update_qc_gt state _)).
-Qed.
-
-Lemma votable_update_round_geq state b:
-  (votable (update state (qc_of b)) b) =
-  (votable state b && (round b >= block_round (qc_vote_data (qc_of b)))).
-Proof.
-by apply/(sameP idP); apply: votable_updateP.
-Qed.
-
-Definition voting_rule state (b: BType) :=
-  let after_update := update state (qc_of b) in
-  if votable (after_update) b then
-    let newState :=
-        mkConsensusState (round b) (preferred_block_round after_update)
-    in
-    (newState, true)
-  else (after_update, false).
-
-Definition voted_on state b := (voting_rule state b).2.
-
-Lemma voted_on_votable state b:
-  voted_on state b = votable (update state (qc_of b)) b.
-Proof.
-rewrite /voted_on /voting_rule.
-by case: (votable (update state (qc_of b)) b) => //.
-Qed.
-
-Lemma voted_br_gt_qcr state b:
-  voted_on state b = true ->
-  round b >= block_round (qc_vote_data (qc_of b)).
-Proof.
-rewrite /voted_on /voting_rule.
-case H: (votable (update state (qc_of b)) b).
-- by move/votable_updateP: H; move/andP => [_ ->].
-- by rewrite /update; case (preferred_block_round state < _).
-Qed.
-
-Lemma ineq_voted_on state b:
-  (voted_on state b) = [&& (round b > last_vote_round state),
-                         (round b >= preferred_block_round state) &
-                         (round b >= block_round (qc_vote_data (qc_of b)))].
-Proof.
-by rewrite voted_on_votable votable_update_round_geq /votable -andbA.
-Qed.
-
-
-Lemma vote_genesis_N: voted_on genesis_state GenesisBlock = false.
-Proof.
-by rewrite voted_on_votable /votable update_eq_lvr /= /genesis_round ltnn.
-Qed.
-
-Definition next_state state b := (voting_rule state b).1.
-
-Lemma next_state_pbr_update state b :
-  preferred_block_round (next_state state b) = preferred_block_round (update state (qc_of b)).
-Proof.
-by rewrite /next_state /voting_rule; case (votable (update state (qc_of b)) b).
-Qed.
-
-Lemma next_state_pbr_geq state b:
-  preferred_block_round state <= preferred_block_round (next_state state b).
-Proof.
-by rewrite next_state_pbr_update update_pbr_geq.
-Qed.
-
-Lemma next_state_lvr_voted state b :
-  reflect (last_vote_round state < last_vote_round (next_state state b)) (voted_on state b).
-Proof.
-rewrite /next_state /voting_rule -voted_on_votable; apply: (iffP idP).
-- move=>H; rewrite (H)=>//=; move:H; rewrite ineq_voted_on.
-  by move/andP=>[-> _].
-- by case: (voted_on state b); rewrite // update_eq_lvr ltnn.
-Qed.
-
-Lemma next_state_lvr_round state b:
-  voted_on state b -> last_vote_round (next_state state b) = round b.
-Proof.
-by rewrite voted_on_votable /next_state /voting_rule=>-> /=.
-Qed.
-
-Lemma next_state_lvr_static state b:
-  ~~ voted_on state b -> last_vote_round (next_state state b) = last_vote_round state.
-Proof.
-rewrite voted_on_votable /next_state /voting_rule.
-by move/negbTE=>->; rewrite update_eq_lvr.
-Qed.
-
-
-Lemma next_state_lvr_if state b:
-  next_state state b =
-  let: pbr:= preferred_block_round (update state (qc_of b)) in
-     if (voted_on state b) then
-       mkConsensusState (round b) pbr
-     else
-       mkConsensusState (last_vote_round state) pbr.
-Proof.
-rewrite /next_state /voting_rule -voted_on_votable /=; case H: (voted_on state b)=> //=.
-by rewrite update_maxn /=.
-Qed.
-
-Lemma next_state_lvr_leq state b:
-  last_vote_round state <= last_vote_round (next_state state b).
-Proof.
-case H: (voted_on state b).
-- by rewrite leq_eqVlt; move/next_state_lvr_voted: H=>->; rewrite orbT.
-- by rewrite /next_state /voting_rule -voted_on_votable H update_eq_lvr.
-Qed.
-
-Lemma next_state_maxn state b:
-  (next_state state b) =
-  let: u_pbr := (maxn (preferred_block_round state) (block_round (qc_vote_data (qc_of b)))) in
-  mkConsensusState
-    (if (round b) >= maxn ((last_vote_round state).+1) u_pbr then round b else last_vote_round state)
-    u_pbr.
-Proof.
-rewrite /next_state /voting_rule update_maxn.
-set pbr:= (maxn (preferred_block_round state) (block_round (qc_vote_data (qc_of b)))).
-rewrite /votable /= -geq_max.
-by case H: (maxn (last_vote_round state).+1 pbr <= round b).
-Qed.
-
-Lemma pbr_next_stateC state b c:
-  preferred_block_round (next_state (next_state state b) c) =
-  preferred_block_round (next_state (next_state state c) b).
-Proof.
-rewrite (next_state_maxn (next_state state c) b) next_state_maxn /=.
-by rewrite !next_state_maxn /= maxnAC.
-Qed.
-
-Lemma voting_next_voted state b :
-  voting_rule state b = (next_state state b, voted_on state b).
-Proof.
-by apply surjective_pairing.
-Qed.
-
-Lemma voting_next_N state b: voted_on (next_state state b) b = false.
-Proof.
-rewrite voted_on_votable votable_update_round_geq /votable.
-rewrite {1}/next_state /voting_rule.
-case H:(votable (update state (qc_of b)) b) => /=; first by rewrite ltnn.
-rewrite /votable -next_state_pbr_update in H.
-by rewrite H andFb.
-Qed.
-
-Lemma voting_update_progress state qc x:
-  voted_on (update state qc) x -> voted_on state x.
-Proof.
-rewrite 2!ineq_voted_on update_maxn /= geq_max.
-by move/andP=>[->]; move/andP =>[H ->]; move/andP: H=>[-> _].
-Qed.
-
-Lemma voting_progress state b x:
-  voted_on (next_state state b) x -> voted_on state x.
-Proof.
-rewrite 2!ineq_voted_on; move/andP=> [Hlvr]; move/andP=> [Hpbr Hbr].
-rewrite (leq_ltn_trans (next_state_lvr_leq _ _) Hlvr).
-by rewrite (leq_trans (next_state_pbr_geq _ _) Hpbr) /=.
-Qed.
-
-Lemma voting_gt state b x:
-  voted_on (next_state state b) x ->
-  ~~ voted_on state b || (round b < round x).
-Proof.
-move=> H; move: (H); rewrite ineq_voted_on; move/andP=> [Hlvr _].
-case I: (voted_on state b)=> //.
-by rewrite (next_state_lvr_round I) in Hlvr.
-Qed.
-
-Lemma non_voted_on_update state b x:
-  ~~ voted_on state b ->
-  voted_on (next_state state b) x = voted_on (update state (qc_of b)) x.
-Proof.
-rewrite next_state_lvr_if; move/negbTE=>->.
-by rewrite update_maxn.
-Qed.
-
-Lemma pbr_update_next state b x:
-  preferred_block_round (update (next_state state b) (qc_of x)) =
-  preferred_block_round (update (update state (qc_of b)) (qc_of x)).
-Proof.
-by rewrite next_state_maxn !update_maxn /=.
-Qed.
-
-Lemma voted_next_update state b x:
-  voted_on (next_state state b) x ->
-  voted_on (update state (qc_of b)) x.
-Proof.
-move=> H; move/voting_progress: (H); rewrite ineq_voted_on; move/andP=> [Hs _].
-move: H; rewrite ineq_voted_on next_state_pbr_update.
-move/andP=>[Hlvr]; move/andP=> [H1 H2].
-by rewrite ineq_voted_on update_eq_lvr Hs H1 H2.
-Qed.
-
-(* TODO: figure out if we want to keep this one, probably obsoleted by *)
-(* comparator reasoning?*)
-Lemma next_stateC state b c:
-  next_state (next_state state b) c =
-  if (~~ voted_on state b || ((round b < round c) &&
-     (block_round (qc_vote_data (qc_of c)) <= round c))) then
-    next_state (update state (qc_of b)) c
-  else
-    (update (next_state state b) (qc_of c)).
-Proof.
-rewrite next_state_lvr_if [next_state (update _ _)_]next_state_lvr_if .
-case H: (~~ voted_on state b).
-- move/idP: (H); move/non_voted_on_update=> ->.
-  by rewrite pbr_update_next (next_state_lvr_static H) update_eq_lvr.
-move/negPn: H=> H; case I: (voted_on (next_state state b) c).
-- move/idP: (I); move/voting_gt; rewrite H /= ltnNge; move/negbTE =>->.
-  move/idP: (I); move/voted_next_update=>->; rewrite pbr_update_next /=.
-  by move/idP: I; move/voting_progress; move/voted_br_gt_qcr=>->.
-move/negbT: (I); rewrite ineq_voted_on negb_and.
-rewrite (next_state_lvr_round H) next_state_pbr_update.
-rewrite ineq_voted_on; move/orP=>[|].
-- by move/negbTE=>->/=; rewrite update_maxn (next_state_lvr_round H) /=.
-move/negbTE=>->; rewrite andbF orFb update_eq_lvr pbr_update_next.
-case J: (round b < round c);
-last by rewrite !update_maxn (next_state_lvr_round H) next_state_pbr_update !update_maxn /=.
-move/negbT: (I); rewrite voted_on_votable /votable.
-move: (H); rewrite ineq_voted_on; move/andP=> [Hlvr]; move/andP=> [Hpbr Hbr].
-rewrite update_maxn (next_state_lvr_round H) J andTb; move/idP: J=> J/=.
-rewrite next_state_maxn /= maxnAC geq_max.
-rewrite [block_round (qc_vote_data (qc_of b)) <= _]leq_eqVlt (leq_ltn_trans Hbr J) orbT andbT.
-rewrite geq_max leq_eqVlt (leq_ltn_trans Hpbr J) orbT andTb; move/negbTE=>-> /=.
-by rewrite !update_maxn /= maxnAC.
-Qed.
-
-Lemma next_state_updateC state qc x:
-  voted_on (update state qc) x ->
-  next_state (update state (qc)) x =
-  update (next_state state x) qc.
-Proof.
-move => H; rewrite /next_state /voting_rule -2!voted_on_votable H.
-by move/voting_update_progress: H=> -> /=; rewrite !update_maxn /= maxnAC.
-Qed.
-
-Lemma voted_on_maxn state b:
-  (voted_on state b) =
-  (round b >= maxn
-               (maxn ((last_vote_round state).+1) (preferred_block_round state))
-               (block_round (qc_vote_data (qc_of b)))).
-Proof.
-by rewrite !geq_max -andbA ineq_voted_on.
-Qed.
-
-(************************************************************)
-(** Voting in Sequence                                     **)
-(************************************************************)
-
-Implicit Type bseq: seq BType.
-
-(* node_processing is a slight modification on a scanleft of the voting rules
-over a seq of block *)
-Fixpoint process_aux state bseq res :=
-  if bseq is x::s then
-    let: (new_state, vote) := (voting_rule state x) in
-    process_aux new_state s ((state, vote) :: res)
-  else
-    (state, rev res).
-
-Definition node_processing state bseq := process_aux state bseq [::].
-
-Lemma size_process_aux state bseq res: size (process_aux state bseq res).2 = size bseq + size res.
-Proof.
-elim:bseq res state => [|x xs IHs] res state.
-- by rewrite size_rev add0n.
-- by rewrite /= voting_next_voted IHs /= addSnnS.
-Qed.
-
-Lemma size_processing state bseq : size (node_processing state bseq).2 = size bseq.
-Proof.
-by rewrite /node_processing size_process_aux addn0.
-Qed.
-
-Lemma processing_aux_state_res_irrel state bseq rs1 rs2:
-  (process_aux state bseq rs1).1 = (process_aux state bseq rs2).1.
-Proof.
-elim: bseq state rs1 rs2 => [|b bs IHb] state rs1 rs2 //=; rewrite voting_next_voted.
-by apply:IHb.
-Qed.
-
-Lemma processing_aux_rcons state bseq r rs:
-  (process_aux state bseq (rcons rs r)).2 =
-  r :: (process_aux state bseq rs).2.
-Proof.
-elim: bseq r rs state =>[| b bs IHb] r rs state => /=.
-- by rewrite rev_rcons.
-- by rewrite voting_next_voted -IHb -rcons_cons.
-Qed.
-
-Lemma processing_aux_rev state bseq res:
-  (process_aux state bseq res).2 =
-  rev res ++ (process_aux state bseq [::]).2.
-Proof.
-move: res bseq state; apply: last_ind=> [|rs r IHr] bseq state.
-- by [].
-- by rewrite processing_aux_rcons IHr rev_rcons.
-Qed.
-
-Lemma processing_aux_cons state b bs:
-  (process_aux state (b::bs) [::]).2 =
-  (state, voted_on state b) :: (process_aux (next_state state b) bs [::]).2.
-Proof.
-rewrite /= voting_next_voted -[[:: (state, voted_on _ _)]]cat0s cats1.
-by rewrite processing_aux_rcons.
-Qed.
-
-Lemma processing_aux_cons2 state b bs:
-  (process_aux state (b::bs) [::]) =
-  let: (f_state, vbs) := (process_aux (next_state state b) bs [::]) in
-  (f_state, (state, voted_on state b) ::vbs).
-Proof.
-rewrite /= voting_next_voted -[[:: (state, voted_on _ _)]]cat0s cats1.
-rewrite [process_aux _ bs [::]]surjective_pairing -processing_aux_cons /=.
-rewrite (processing_aux_state_res_irrel _ _ [::] [:: (state, voted_on state b)]).
-by rewrite voting_next_voted -surjective_pairing.
-Qed.
-
-Lemma node_processing_cons state b bs:
-  (node_processing state (b::bs)).2 =
-  (state, voted_on state b) :: (node_processing (next_state state b) bs).2.
-Proof.
-by rewrite processing_aux_cons.
-Qed.
-
-Lemma node_processing_cons2 state b bs:
-  (node_processing state (b::bs)) =
-  let: (final_state, bsvotes) := node_processing (next_state state b) bs in
-  (final_state, (state, voted_on state b)::bsvotes).
-Proof.
-by  rewrite /node_processing processing_aux_cons2.
-Qed.
-
-Lemma node_processing_cons1 state b bs:
-  (node_processing state (b::bs)).1 =
-  (node_processing (next_state state b) bs).1.
-Proof.
-case: bs state b=>[|x s ]=>state b; rewrite node_processing_cons2 //=.
-by rewrite [node_processing _ _]surjective_pairing /=.
-Qed.
-
-Lemma node_processing_cat_cps state bs1 bs2 :
-  (node_processing state (bs1 ++ bs2)) =
-  let: (state1, seq1) := (node_processing state bs1) in
-  let: (state2, seq2) := (node_processing state1 bs2) in
-  (state2, seq1 ++ seq2).
-Proof.
-elim: bs1 state =>[| b bs IHb] state /=.
-- by rewrite {2}[node_processing _ _]surjective_pairing -surjective_pairing.
-rewrite 2!node_processing_cons2 IHb [node_processing (next_state _ _) _]surjective_pairing /=.
-by rewrite [node_processing _  _]surjective_pairing.
-Qed.
-
-Lemma node_processing_rcons state bs b:
-  (next_state (node_processing state bs).1 b) =
-  (node_processing state (rcons bs b)).1.
-Proof.
-rewrite -cats1 node_processing_cat_cps /=.
-rewrite {2}[node_processing _ _]surjective_pairing /=.
-rewrite [node_processing _ [::b]]surjective_pairing /=.
-by rewrite node_processing_cons1 /=.
-Qed.
-
-Lemma voting_progress_seq state bs b:
-  voted_on (node_processing state bs).1 b -> voted_on state b.
-Proof.
-elim: bs state b => [|x s IHs] state b //=.
-rewrite node_processing_cons1.
-move/IHs; apply voting_progress.
-Qed.
-
-(************************************************************)
-(** Consensus State Comparators                            **)
-(************************************************************)
-
-Definition comparator state1 :=
-  maxn (last_vote_round state1).+1 (preferred_block_round state1).
-
-Definition state_compare state1 state2 :=
-  comparator state1 <= comparator state2.
-
-Delimit Scope state_scope with STATE.
-Open Scope state_scope.
-
-Notation "state1 <% state2" := (state_compare state1 state2) (at level 40) :state_scope.
-
-Lemma voting_comparator state x:
-  (voted_on state x) ->
-  (comparator (next_state state x) = (round x).+1).
-Proof.
-rewrite next_state_lvr_if fun_if /comparator /= =>H.
-rewrite H; apply/maxn_idPl; move/idP:H; rewrite voted_on_votable.
-by move/andP=>[_ H]; apply ltnW; rewrite ltnS.
-Qed.
-
-Lemma non_voting_comparator state x:
-  ~~ voted_on state x ->
-  comparator (next_state state x) = maxn (comparator state) (block_round (qc_vote_data (qc_of x))).
-Proof.
-move=>Hnv; rewrite next_state_lvr_if; move/negbTE: (Hnv)=>->.
-by rewrite /comparator update_maxn /= maxnA.
-Qed.
-
-Lemma voting_comparator_eq state b:
-    (voted_on state b) =
-    ((comparator state <= round b) && (block_round (qc_vote_data (qc_of b)) <= round b))
-    .
-Proof.
-by rewrite /comparator geq_max -andbA -ineq_voted_on.
-Qed.
-
-Lemma voting_gt_compare state1 state2 x:
-  state1 <% state2 -> voted_on state2 x -> voted_on state1 x.
-Proof.
-move=> H; rewrite 2!voted_on_maxn; apply leq_trans.
-rewrite geq_max leq_maxr leq_max andbT.
-by apply/orP; left.
-Qed.
-
-Lemma voting_next_gt state x:
-  state <% (next_state state x).
-Proof.
-rewrite next_state_lvr_if.
-case Hx:(voted_on state x); rewrite /state_compare /=.
-- move/idP: Hx; rewrite voted_on_maxn.
-  rewrite leq_max geq_max; move/andP=> [H _].
-  by apply/orP; left; apply ltnW.
-rewrite update_maxn /= leq_max 2!geq_max ltnS leqnn andTb.
-rewrite leq_maxl andbT leq_max.
-case I: (last_vote_round state < preferred_block_round state);
-first by rewrite orTb orbT.
-move/negbT: I; rewrite ltnNge; move/negPn=> H.
-by rewrite orFb; apply/orP; left; apply ltnW.
-Qed.
-
-Lemma voting_processing_gt state bs:
-  state <% (node_processing state bs).1.
-Proof.
-elim: bs state=> [|b s IHs] state /=; first by rewrite /state_compare.
-rewrite node_processing_cons1; move:(@voting_next_gt state b).
-move/leq_trans; apply; apply IHs.
-Qed.
-
-Lemma voting_next_inner state1 state2 x:
-  state1 <% state2 ->
-  (next_state state1 x) <% (next_state state2 x).
-Proof.
-move => H12.
-case H2: (voted_on state2 x).
-- rewrite /state_compare (voting_comparator H2).
-  move/(voting_gt_compare H12): H2; move/voting_comparator=>->.
-  by apply: ltnSn.
-case H1: (voted_on state1 x).
-- rewrite /state_compare (voting_comparator H1).
-  rewrite /comparator; move/negbT: (H2); rewrite voted_on_votable.
-  rewrite /votable /= next_state_pbr_update next_state_lvr_if H2 /=.
-  rewrite negb_and -leqNgt -ltnNge leq_max.
-  move/orP=>[|->]; last by rewrite orbT.
-  by rewrite update_maxn /= ltnS =>->.
-rewrite 2!next_state_lvr_if H1 H2.
-move: H12; rewrite /state_compare /comparator 2!update_maxn /=.
-rewrite !maxnA=>H12; rewrite geq_max leq_max H12 orTb andTb.
-by rewrite leq_max leqnn orbT.
-Qed.
-
-Lemma voting_processing_inner state1 state2 bs:
-  state1 <% state2 ->
-  (node_processing state1 bs).1 <% (node_processing state2 bs).1.
-Proof.
-move: state1 state2; elim bs => [|b s IHs]=> state1 state2 H12 //.
-by rewrite 2!node_processing_cons1 IHs // voting_next_inner.
-Qed.
-
-(************************************************************)
-(** Sequence of elements which a node voted on             **)
-(************************************************************)
-
-Definition voted_in_processing state bseq :=
-  mask (unzip2 (node_processing state bseq).2) bseq.
-
-Lemma voted_in_processing_cat_cps state bs1 bs2:
-  (voted_in_processing state (bs1 ++ bs2)) =
-  let: b1 := (voted_in_processing state bs1) in
-  let: b2 := (voted_in_processing (node_processing state bs1).1 bs2) in
-  b1 ++ b2.
-Proof.
-rewrite /voted_in_processing node_processing_cat_cps /=.
-rewrite 2![node_processing _ _]surjective_pairing /=.
-rewrite -mask_cat; last by rewrite size_map size_processing.
-by rewrite -map_cat /unzip2.
-Qed.
-
-Lemma voted_in_processing_cons state b bs:
-  (voted_in_processing state (b::bs)) =
-  (nseq (voted_on state b) b ++ (voted_in_processing (next_state state b) bs)).
-Proof.
-by rewrite /voted_in_processing node_processing_cons mask_cons.
-Qed.
-
-Lemma comparatorC state b c:
-  comparator (next_state (next_state state b) c) =
-  comparator (next_state (next_state state c) b).
-Proof.
-rewrite next_state_maxn maxnA -/(comparator (next_state _ _)).
-rewrite [next_state (next_state _ _) _]next_state_maxn maxnA.
-rewrite -/(comparator (next_state _ _)) 2!geq_max 2!next_state_pbr_update 2!update_maxn /=.
-rewrite 2![comparator {|last_vote_round := _; preferred_block_round:= _|}]/comparator /= maxnAC.
-case Hc: (voted_on state c); [rewrite (next_state_lvr_round Hc) (voting_comparator Hc) (voted_br_gt_qcr Hc) andbT
-  | move/negbT/next_state_lvr_static: (Hc)=>->; rewrite (non_voting_comparator (negbT Hc)) geq_max];
-case Hb: (voted_on state b); [ rewrite (next_state_lvr_round Hb) (voting_comparator Hb) (voted_br_gt_qcr Hb) andbT
-  | move/negbT/next_state_lvr_static: (Hb)=>->; rewrite (non_voting_comparator (negbT Hb)) geq_max
-  | rewrite (next_state_lvr_round Hb) (voting_comparator Hb) (voted_br_gt_qcr Hb) andbT
-  | move/negbT/next_state_lvr_static: (Hb)=>->; rewrite (non_voting_comparator (negbT Hb)) geq_max].
-- case Hbc: (round b == round c); first by move/eqP: Hbc; move=><-; rewrite ltnn.
-  by move/negbT: (Hbc); rewrite neq_ltn; move/orP=>[Hltn|Hltn]; rewrite Hltn /=; move: Hltn; rewrite ltnNge leq_eqVlt;
-  [rewrite eq_sym|]; rewrite Hbc orFb; move/negbTE=>->/=.
-- move: (Hc); rewrite voting_comparator_eq; move/andP=>[Hcpc Hbrc] /=.
-  rewrite Hcpc; move/negbT: (Hb); rewrite voting_comparator_eq negb_and.
-  case Hbrb: ((block_round (qc_vote_data (qc_of b))) <= round b); [rewrite orbF andbT andTb -ltnNge => Hcpb | rewrite andbF andTb => _ ].
-  - by rewrite ltnNge; move/ltnW: (leq_trans Hcpb Hcpc)=> Hbc; rewrite Hbc (leq_trans Hbrb Hbc) /=.
-  move/negbT: Hbrb; rewrite -ltnNge=> Hbrb; case Hqbc: (block_round (qc_vote_data (qc_of b)) <= round c); first by [].
-  move/negbT: Hqbc; rewrite -ltnNge=> Hqbc; rewrite [maxn (round c).+1 _]maxnCA; move/maxn_idPr: (Hqbc)=>->.
-  rewrite 2!maxnA -/(comparator state) maxnAC; move/ltnW: (leq_ltn_trans Hcpc Hqbc); move/maxn_idPr=>->.
-  move: (leq_maxr (last_vote_round state).+1 (preferred_block_round state)); rewrite -/(comparator state)=> Hprcsc.
-  by rewrite maxnAC; move: (leq_ltn_trans (leq_trans Hprcsc Hcpc) Hqbc); move/ltnW/maxn_idPr=>->.
-- move: (Hb); rewrite voting_comparator_eq; move/andP=>[Hcpb Hbrb] /=.
-  rewrite Hcpb; move/negbT: (Hc); rewrite voting_comparator_eq negb_and.
-  case Hbrc: ((block_round (qc_vote_data (qc_of c))) <= round c);
-    [rewrite orbF andbT andTb -ltnNge => Hcpc | rewrite andbF andTb => _ ].
-  - by rewrite ltnNge; move/ltnW: (leq_trans Hcpc Hcpb)=> Hbb; rewrite Hbb (leq_trans Hbrc Hbb) /=.
-  move/negbT: Hbrc; rewrite -ltnNge=> Hbrc; case Hqbb: (block_round (qc_vote_data (qc_of c)) <= round b); first by [].
-  move/negbT: Hqbb; rewrite -ltnNge=> Hqbb; rewrite maxnAC; rewrite  [maxn (round b).+1 _]maxnCA; move/maxn_idPr: (Hqbb)=>->.
-  rewrite 2!maxnA -/(comparator state) [maxn (maxn (comparator _) _) _]maxnAC; move/ltnW: (leq_ltn_trans Hcpb Hqbb); move/maxn_idPr=>->.
-  move: (leq_maxr (last_vote_round state).+1 (preferred_block_round state)); rewrite -/(comparator state)=> Hprcsb.
-  by rewrite maxnAC; move: (leq_ltn_trans (leq_trans Hprcsb Hcpb) Hqbb); move/ltnW/maxn_idPr=>->.
-by rewrite andbAC -voting_comparator_eq Hc andFb andbAC -voting_comparator_eq Hb andFb.
-Qed.
-
-Lemma comparator_next state1 state2 b:
-  comparator state1 = comparator state2
-  -> comparator (next_state state1 b) = comparator (next_state state2 b).
-Proof.
-move=> H12; case H1: (voted_on state1 b); move: (H1); rewrite voting_comparator_eq H12 -voting_comparator_eq=> H2.
-- by rewrite (voting_comparator H1) (voting_comparator H2).
-by rewrite (non_voting_comparator (negbT H1)) (non_voting_comparator (negbT H2)) H12.
-Qed.
-
-Lemma comparator_processing state1 state2 bseq:
-  comparator state1 = comparator state2
-  -> comparator (node_processing state1 bseq).1 = comparator (node_processing state2 bseq).1.
-Proof.
-elim: bseq state1 state2 =>[| x s IHs] state1 state2 H12 //.
-by rewrite 2!node_processing_cons1 (IHs _ _ (comparator_next x H12)).
-Qed.
-
-Lemma comparator_push_right state bs b:
-  comparator (node_processing state (b::bs)).1 = comparator (node_processing state (rcons bs b)).1.
-Proof.
-elim: bs state b => [|x s IHs] state b //=.
-rewrite -rcons_cons -node_processing_rcons; move/comparator_next: (IHs state x)=>->.
-rewrite -node_processing_rcons comparatorC 2!node_processing_rcons.
-rewrite node_processing_cons1 IHs -node_processing_cons1 -rcons_cons -node_processing_rcons.
-by move/comparator_next: (IHs state b)=>->; rewrite node_processing_rcons.
-Qed.
-
-Lemma next_state_repeat state b:
-  (next_state (next_state state b) b) = (next_state state b).
-Proof.
-rewrite next_state_lvr_if voting_next_N update_maxn next_state_pbr_update update_maxn  /= -maxnA maxnn.
-rewrite -/(preferred_block_round {| last_vote_round := last_vote_round state;
-  preferred_block_round := maxn (preferred_block_round state) (block_round (qc_vote_data (qc_of b))) |}).
-rewrite -update_maxn -next_state_pbr_update.
-have H: forall s, s = {| last_vote_round := (last_vote_round s);
-                    preferred_block_round:= (preferred_block_round s)|}; first by case.
-by rewrite {3}(H (next_state state b)).
-Qed.
-
-Lemma comparator_repeat state b:
-  comparator (next_state (next_state state b) b) =
-  comparator (next_state state b).
-Proof.
-by rewrite next_state_repeat.
-Qed.
-
-Lemma comparator_predC1 state bs b:
-  b \in bs ->
-  comparator (node_processing state bs).1 =
-  comparator (node_processing (next_state state b) (filter (predC1 b) bs)).1.
-Proof.
-elim: bs state b =>[|x s IHs] // state b.
-rewrite in_cons node_processing_cons1; case Hx: (b \in s).
-- move=>_; rewrite (IHs _ _ Hx); case Hbx: (b == x).
-  - by move/eqP: Hbx=>->; rewrite (comparator_processing _ (comparator_repeat _ _)) {2}/filter /predC1 /= eq_refl /=.
-   by rewrite (comparator_processing _ (comparatorC state x b)) {2}/filter /predC1 /= eq_sym Hbx /= -node_processing_cons1.
-rewrite orbF=> Hbx; move/negbT: Hx; rewrite -not_in_all_predC1; move/all_filterP; rewrite /filter /predC1 /= eq_sym Hbx /==>->.
-by move/eqP: Hbx=><-.
-Qed.
-
-Lemma comparator_orderfree state bs1 bs2:
-  bs1 =i bs2 ->
-  comparator (node_processing state bs1).1 = comparator (node_processing state bs2).1.
-Proof.
-elim: bs1 state bs2 => [|x s IHs] state bs2 H12 //; last rewrite node_processing_cons1.
-- by case: bs2 H12 => [|x2 s2] H12 //; move: (H12 x2); rewrite in_nil in_cons eq_refl.
-case Hx: (x \in s).
-- have: s=ibs2; first by move=> y; rewrite -H12 in_cons; move: Hx; case Hxy: (y == x); [move/eqP: Hxy=>->->| rewrite orFb].
-  move: (predC1_split Hx); move/IHs=>->; rewrite node_processing_cons1 (comparator_processing _ (comparator_repeat state x)).
-  rewrite -node_processing_cons1; move/IHs: (predC1_split Hx)=><-; apply IHs.
-have: s=i (filter (predC1 x) bs2); first move => y.
-- move: (H12 y); rewrite in_cons mem_filter /predC1 /=; case Hyx: (y == x); by [move/eqP: Hyx=>->| rewrite andTb orFb].
-  by move/IHs=>->; move: (mem_head x s); rewrite H12; move/comparator_predC1=>->.
-Qed.
-
-Lemma voted_in_processing_repeat state b bs:
-  voted_in_processing (next_state state b) (b:: bs) =
-  voted_in_processing (next_state state b) (bs).
-Proof.
-rewrite /voted_in_processing !node_processing_cons !mask_cons.
-by rewrite voting_next_N next_state_repeat.
-Qed.
-
-Lemma voted_in_processing_comparison state1 state2 bs:
-  comparator state1 = comparator state2 ->
-  voted_in_processing state1 bs = voted_in_processing state2 bs.
-Proof.
-elim: bs state1 state2=>[| x s IHs] state1 state2 H12 //.
-rewrite /voted_in_processing 2!node_processing_cons 2!mask_cons.
-rewrite -/(map snd) -/unzip2 -2!/(voted_in_processing (next_state _ x) s).
-rewrite (IHs _ _ (comparator_next x H12)) /=.
-by rewrite 2!voting_comparator_eq H12.
-Qed.
-
-Lemma voted_in_predC1 state b bs:
-  voted_in_processing (next_state state b) (bs) =
-  voted_in_processing (next_state state b) (filter (predC1 b) bs).
-Proof.
-elim: bs state b =>[| x s IHs] state b //=.
-case Hbx: (x == b)=>/=.
-- move/eqP: Hbx=>->; rewrite {1}/voted_in_processing node_processing_cons mask_cons.
-  rewrite next_state_repeat voting_next_N -/(map snd) -/unzip2.
-  by rewrite -/(voted_in_processing (next_state state b) s) IHs.
-rewrite /voted_in_processing 2![(node_processing _ (x:: _)).2]node_processing_cons.
-rewrite 2!mask_cons -/(map snd) -/unzip2 -/(voted_in_processing _ s).
-rewrite (voted_in_processing_comparison _ (comparatorC _ _ _)) IHs.
-by rewrite (voted_in_processing_comparison _ (comparatorC _ _ _)).
-Qed.
-
-Lemma voted_in_rundup state bs:
-  voted_in_processing state bs = voted_in_processing state (rundup bs).
-Proof.
-elim: bs state =>[| x s IHs] state //=.
-rewrite /voted_in_processing 2!node_processing_cons /unzip2 map_cons mask_cons.
-rewrite -/(voted_in_processing (next_state state x) s) IHs .
-rewrite mask_cons -/(map snd) -/unzip2 -/(voted_in_processing (next_state state x) _).
-by rewrite -voted_in_predC1.
-Qed.
-
-Lemma voted_in_processing_state_orderfree state bs1 bs2 bseq:
-  bs1 =i bs2 ->
-  voted_in_processing (node_processing state bs1).1 bseq =
-  voted_in_processing (node_processing state bs2).1 bseq.
-Proof.
-move=> H; apply (voted_in_processing_comparison _ (comparator_orderfree _ H)).
-Qed.
-
-Lemma voted_in_processing_idx state bseq b:
-  (b \in (voted_in_processing state bseq)) =
-  (voted_on (nth state (unzip1 (node_processing state bseq).2) (index b bseq) ) b && (b \in bseq)).
-Proof.
-rewrite voted_in_rundup.
-elim: bseq b state =>[| bb bbs IHbb] b state /=.
-- by rewrite in_nil andbF.
-rewrite /voted_in_processing /= 2!node_processing_cons /unzip2 mask_cons -/(map snd) /=.
-case H: (bb == b).
-- move/eqP: H=> ->; rewrite in_cons eqxx.
-  case H2: (voted_on state b); first by rewrite in_cons eqxx orTb andbT.
-  rewrite /=; apply: negbTE; apply: contraT; move/negPn=>H.
-  by move: (mem_mask H); rewrite mem_filter /= eq_refl.
-rewrite mem_cat mem_nseq in_cons eq_sym H andbF 2!orFb.
-rewrite -/unzip2 -/(voted_in_processing (next_state state bb) _).
-rewrite -voted_in_predC1 IHbb /=; case Hbbs: (b\in bbs); last by rewrite 2!andbF.
-rewrite (nth_in_default_irrel (next_state state bb) state _); first by [].
-by rewrite size_map size_processing index_mem.
-Qed.
-
-(************************************************************)
-(** Node Aggregation                                       **)
-(************************************************************)
-
-
-Definition node_aggregator bseq :=
-  (foldl (fun stateNvote => voting_rule stateNvote.1) (genesis_state,false) bseq).1.
-
-
-Definition commit_rule state (qc: QC)(bround: nat) :=
-  let: potential_commit_round := (parent_block_round (qc_vote_data qc)) in
-  if (potential_commit_round.+1 == (block_round (qc_vote_data qc))) &&
-        ((block_round (qc_vote_data qc)).+1 == bround) then
-    Some(potential_commit_round)
-  else None.
+Lemma btExtendV bt b :
+  valid (btExtend bt b) -> valid bt.
+Proof.
+rewrite/btExtend; case: ifP.
+by case: ifP=>//=; rewrite valid_undef.
+by move=>Nd; rewrite validPtUn Nd //==>[/andP] [].
+Qed.
+
+Lemma btExtendV_comm bt a b :
+  valid (btExtend (btExtend bt a) b) =
+  valid (btExtend (btExtend bt b) a).
+Proof.
+rewrite/btExtend; case: ifP; case: ifP; case: ifP; case: ifP;
+move=>A B C D.
+by rewrite D C B.
+by rewrite D dom_undef in_nil validPtUn valid_undef.
+by rewrite dom_undef in D.
+by rewrite dom_undef in D.
+- case: ifP; case: ifP.
+  case: ifP=>X Y Z.
+  by rewrite Y X in A; rewrite A in C.
+  by rewrite find_undef in Z.
+  by move=>X; move: D; rewrite domPtUn inE X Bool.orb_false_r=>/andP [] _;
+     move/eqP=>->_ ; rewrite !validPtUn !inE.
+  case: ifP=>X Y Z.
+  by rewrite Y X in A; rewrite A in C.
+  by rewrite Y X dom_undef in A.
+  move=>X; move: D; rewrite domPtUn inE X Bool.orb_false_r=>/andP[]->.
+    move/eqP=>E; move: A; rewrite X domPtUn inE=>/andP[]V _.
+    move: B; rewrite E findUnR; last by move: V; rewrite !validPtUn.
+    rewrite X findPt //==>/eqP []E'; subst b;
+    by rewrite findUnR ?V //= X findPt //==>/eqP [].
+- case: ifP.
+  case: ifP=>X Y //=.
+  by move: D; rewrite domPtUn inE Y=>/andP[] V _;
+    move: B; rewrite findUnR ?V //= Y X.
+  by move=>X; move: D; rewrite domPtUn inE X Bool.orb_false_r=>/andP [] V;
+    move/eqP=>E; move: A; rewrite X E domPtUn inE eq_refl Bool.orb_true_l;
+    move: V; rewrite !validPtUn C X !Bool.andb_true_r//==>->.
+- case: ifP; case: ifP=>//=.
+  case: ifP=>X Y Z=>//=.
+  by rewrite Y X in A; rewrite A in C.
+  move=>X; move: D; rewrite domPtUn inE X Bool.orb_false_r=>/andP [] V.
+  move/eqP=>E; move: B; rewrite E !findUnR;
+    do? by move:V; rewrite !validPtUn C X //=.
+  by rewrite X !findPt //= eq_sym=>->.
+- case: ifP.
+  case: ifP=>X Y; move: B; rewrite findUnR.
+  by case: ifP; [rewrite X | rewrite Y].
+  by move: D; rewrite domPtUn inE validPtUn Y C //==>/andP[].
+  by case: ifP; rewrite join_undefR.
+  by move: D; rewrite domPtUn inE validPtUn Y C //==>/andP[].
+  by rewrite joinA (joinC (#a \\-> _) (#b \\-> _)) -joinA;
+     rewrite validPtUn inE D //= Bool.andb_false_r valid_undef.
+- rewrite D in A *; case: ifP=>//=.
+  rewrite findUnR. by rewrite C B.
+  by move: A; rewrite domPtUn inE=>/andP[].
+- rewrite D in A *.
+  by rewrite validPtUn D !validPtUn A D //= !Bool.andb_true_r.
+- case: ifP; case: ifP; do? by rewrite join_undefR.
+  case: ifP=>X Y Z.
+  by rewrite Z in B.
+  by rewrite find_undef in Z.
+  move=>X; rewrite findUnR. by rewrite C B.
+  by move: A; rewrite X domPtUn validPtUn inE X C //=;
+     rewrite Bool.orb_true_r !Bool.andb_true_r.
+- case: ifP.
+  case: ifP=>X Y; first by rewrite Y X C in A.
+  by rewrite !join_undefR.
+  rewrite joinA (joinC (#a \\-> _) (#b \\-> _)) -joinA.
+  suff: (# a \\-> a \+ bt) = um_undef by move=>->.
+  by apply invalidE; rewrite validPtUn C Bool.andb_false_r.
+- case: ifP; case: ifP=>X Y; do? by rewrite X C in B.
+  by rewrite find_undef in Y.
+  by rewrite X dom_undef in_nil in B.
+- case: ifP; first by rewrite !validPtUn A C D //= !Bool.andb_true_r.
+  move: B; rewrite domPtUn inE C Bool.orb_false_r=>/andP[]V /eqP E.
+  contradict D.
+  rewrite domPtUn inE E eq_refl Bool.orb_true_l Bool.andb_true_r.
+  by move: V; rewrite !validPtUn C //= Bool.andb_true_r=>/andP[]->.
+- case: ifP=>X.
+  contradict D.
+    rewrite domPtUn inE A Bool.orb_true_r validPtUn C //=.
+    case V: (valid bt)=>//=.
+    move: (invalidE bt); rewrite V //=; case=>Z _.
+    have T: true by []. specialize (Z T).
+    by move: Z A=>->; rewrite dom_undef in_nil.
+  by rewrite joinA (joinC (#b \\-> _)) -joinA !validPtUn //=;
+     rewrite A //= Bool.andb_false_r valid_undef !Bool.andb_false_l.
+by rewrite !joinA (joinC (#b \\-> _) (#a \\-> _)).
+Qed.
+
+Lemma btExtendV_fold1 bt bs b :
+  valid (foldl btExtend bt (rcons bs b)) -> valid (foldl btExtend bt bs).
+Proof.
+rewrite -cats1 foldl_cat /= {1}/btExtend; case: ifP.
+case: ifP=>_ _ =>//=; last by rewrite valid_undef.
+by move=>_; rewrite validPtUn /= =>/andP[H _].
+Qed.
+
+Lemma btExtendV_fold bt xs ys :
+  valid (foldl btExtend bt (xs ++ ys)) -> valid (foldl btExtend bt xs).
+Proof.
+elim/last_ind: ys=>[|ys y Hi]; first by rewrite cats0.
+by rewrite foldl_cat; move/btExtendV_fold1; rewrite -foldl_cat; apply Hi.
+Qed.
+
+Lemma btExtendV_fold_xs bt xs :
+  valid (foldl btExtend bt xs) -> valid bt.
+Proof.
+have X: xs = ([::] ++ xs) by rewrite cat0s.
+by rewrite X; move/btExtendV_fold.
+Qed.
+
+Lemma btExtendV_fold_dup bt xs a b :
+  valid (foldl btExtend bt (rcons xs a)) ->
+  b \in xs -> #a = #b -> a = b.
+Proof.
+elim/last_ind: xs=>[|xs x H]//=.
+rewrite -!cats1 !foldl_cat //=.
+have E: (btExtend (btExtend (foldl btExtend bt xs) a) x) =
+        foldl btExtend bt (rcons (rcons xs a) x)
+by rewrite -!cats1 -catA !foldl_cat //=.
+rewrite btExtendV_comm E=>V; move: (btExtendV_fold1 V)=>V0.
+specialize (H V0); rewrite mem_cat inE=>/orP; case=>//=.
+move/eqP=>Eq; subst x; move=>Hh.
+case X: (a == b); first by move/eqP: X.
+contradict V.
+rewrite -!cats1 !foldl_cat //=.
+move: (btExtendV_fold1 V0)=>V1.
+rewrite{1}/btExtend; case: ifP.
+- case: ifP.
+  rewrite{5}/btExtend; case: ifP.
+  case: ifP; last by rewrite valid_undef.
+  rewrite -Hh.
+  move=>A B C _; contradict C.
+  by rewrite{1}/btExtend B A; move/eqP: A=>-> /eqP [] Y;
+     rewrite Y eq_refl in X.
+  move=>A B C D; move: B.
+  by rewrite{1}/btExtend A -Hh findPtUn ?D //==>/eqP [] Y;
+     rewrite Y eq_refl in X.
+  by rewrite valid_undef.
+move=>D; rewrite{1}/btExtend.
+case: ifP.
+case: ifP; last by rewrite join_undefR valid_undef.
+by move=>B A; rewrite -Hh validPtUn A //= Bool.andb_false_r.
+by rewrite -Hh joinA (joinC _ (foldl btExtend _ _));
+   move=>_; apply/negP; apply invalidE; rewrite pts_undef join_undefR.
+Qed.
+
+Lemma btExtendH bt b : valid bt -> validH bt -> validH (btExtend bt b).
+Proof.
+move=>V H z c; rewrite /btExtend.
+case: ifP=>X.
+- case: ifP=>_; by [move/H | rewrite find_undef].
+rewrite findUnL ?validPtUn ?V ?X//.
+case: ifP=>Y; last by move/H.
+rewrite domPtK inE in Y; move/eqP: Y=>Y; subst z.
+by rewrite findPt; case=>->.
+Qed.
+
+Lemma btExtendH_fold bt bs :
+  validH bt -> valid (foldl btExtend bt bs) ->
+  validH (foldl btExtend bt bs).
+Proof.
+move=>Vh V'; elim/last_ind: bs V' =>[|xs x Hi] V'; first done.
+move: (btExtendV_fold1 V')=>V; move: (Hi V).
+rewrite -cats1 foldl_cat /= {2}/btExtend; case: ifP.
+case: ifP=>//=; by move: validH_undef.
+move=>D H; rewrite/validH=>h b; rewrite findUnR ?validPtUn ?V ?D //=.
+case: ifP; first by move: (H h b).
+by rewrite findPt2; case: ifP=>//= /andP[/eqP ->] _ _ [] ->.
+Qed.
+
+Lemma btExtendIB bt b :
+  validH bt -> valid (btExtend bt b) -> has_init_block bt ->
+  has_init_block (btExtend bt b).
+Proof.
+move=>Vh V'; rewrite /btExtend/has_init_block=>Ib.
+move: (btExtendV V')=>V; case: ifP=>X; last first.
+by move: (find_some Ib)=>G; rewrite findUnR ?validPtUn ?X ?V //= G Ib.
+case: ifP=>//=.
+case: (um_eta X)=>v [F _].
+rewrite F=>/eqP; move: (Vh _ _ F)=>H Neq.
+contradict V'; rewrite/btExtend X; case: ifP.
+by rewrite F=>/eqP [] E; subst v.
+by rewrite valid_undef.
+Qed.
+
+Lemma btExtendIB_fold bt bs :
+  validH bt -> valid (foldl btExtend bt bs) -> has_init_block bt ->
+  has_init_block (foldl btExtend bt bs).
+Proof.
+move=>Vh V'; rewrite/has_init_block=>iB.
+elim/last_ind: bs V'=>[|xs x Hi]; first done.
+rewrite -cats1 foldl_cat /= {1}/btExtend; case: ifP.
+- case: ifP; last by rewrite valid_undef.
+  by move=>F D V; rewrite{1}/btExtend D F; apply Hi.
+move=>Nd; rewrite validPtUn Nd /==>/andP[V _].
+rewrite{1}/btExtend Nd findUnR ?validPtUn ?V ?Nd //=.
+by move: (find_some (Hi V)) (Hi V)=>-> ->.
+Qed.
+
+Lemma in_ext bt b : valid (btExtend bt b) -> validH bt -> b ∈ btExtend bt b.
+Proof.
+move=>V' Vh; rewrite/btHasBlock/btExtend;
+move: (btExtendV V')=>V; case: ifP=>//=; last first.
+- rewrite domUn inE ?validPtUn ?V //==>D; rewrite D domPt inE/=.
+  apply/andP; split.
+  by apply/orP; left.
+  by rewrite findUnL ?validPtUn ?V ?D //; rewrite domPt inE /=;
+      case: ifP=>/eqP//= _; rewrite findPt /=.
+move=>D; case: ifP.
+by rewrite D=>/eqP ->; apply /andP; split=>//=.
+case: (um_eta D)=>b' [] F' _; move: (Vh _ _ F')=>H F.
+rewrite F' in F; contradict V'.
+rewrite/btExtend D; case: ifP; last by rewrite valid_undef.
+by rewrite F' F.
+Qed.
+
+Lemma btExtend_dom bt b :
+  valid (btExtend bt b) -> {subset dom bt <= dom (btExtend bt b)}.
+Proof.
+move=>V' z; rewrite/btExtend; case:ifP=>C//=D.
+case: ifP=>//= F.
+by contradict V'; rewrite/btExtend C F valid_undef.
+move: (btExtendV V')=>V.
+by rewrite domUn inE andbC/= validPtUn/= V D/= C orbC.
+Qed.
+
+Lemma btExtend_dom_fold bt bs :
+  valid (foldl btExtend bt bs) -> {subset dom bt <= dom (foldl btExtend bt bs)}.
+Proof.
+move=>V z; elim/last_ind: bs V=>[|xs x Hi]=>//.
+move=>V'; move: (btExtendV_fold1 V')=>V D; specialize (Hi V D).
+rewrite -cats1 foldl_cat /=; apply btExtend_dom=>//=.
+by move: V'; rewrite -cats1 foldl_cat /=.
+Qed.
+
+Lemma btExtend_find bt z h b :
+  valid (btExtend bt z) ->
+  h \in dom bt ->
+  find h (btExtend bt z) = Some b ->
+  find h bt = Some b.
+Proof.
+move=>V' D; move: (btExtendV V')=>V.
+rewrite/btExtend; case:ifP=>C.
+case: ifP=>//=C'; first by rewrite find_undef.
+rewrite findUnR ?validPtUn ?V ?C //; case: ifP=>//=.
+by rewrite D.
+Qed.
+
+Lemma btExtend_find_fold bt h b bs :
+  valid (foldl btExtend bt bs) ->
+  h \in dom bt ->
+  find h (foldl btExtend bt bs) = Some b ->
+  find h bt = Some b.
+Proof.
+move=>V' D.
+elim/last_ind: bs V'=>[|xs x Hi]=>//.
+move=>V'; move: (btExtendV_fold1 V')=>V; move: V'.
+rewrite -cats1 foldl_cat /= =>X.
+specialize (Hi V); rewrite{1}/btExtend.
+case: ifP.
+case: ifP; last by rewrite find_undef.
+by move=>_ _ ; apply Hi.
+move=>Nd; rewrite findUnR ?validPtUn ?Nd ?V //.
+case: ifP; first by move=>_; apply Hi.
+move=>Nd'; rewrite findPt2 //=; case: ifP=>//=.
+by move: (btExtend_dom_fold V D); rewrite Nd'.
+Qed.
+
+Lemma btExtend_fold_in_either bt xs b :
+  b ∈ (foldl btExtend bt xs) ->
+  b ∈ bt \/ b \in xs.
+Proof.
+elim/last_ind: xs=>[|xs x H]; first by left.
+rewrite -cats1 foldl_cat //= {1}/btExtend.
+case: ifP; last first.
+- move=>D; rewrite/btHasBlock=>/andP [].
+  rewrite domPtUn inE=>/andP[]Z/orP; case.
+  * move/eqP=>Hh; rewrite Hh findPtUn; last by rewrite -Hh.
+    move/eqP=>[]E; subst x; right.
+    by rewrite mem_cat inE eq_refl Bool.orb_true_r.
+  move=>A; rewrite findPtUn2 ?Z //=; case: ifP.
+  by move=>_ /eqP[]->; right; rewrite mem_cat inE eq_refl Bool.orb_true_r.
+  move=>_ B; have X: (b ∈ foldl btExtend bt xs) by rewrite/btHasBlock A B.
+  move: (H X); case; first by rewrite/btHasBlock=>->; left.
+  by move=>M; right; rewrite mem_cat M Bool.orb_true_l.
+case: ifP.
+move=>_ _ M; case: (H M); first by left.
+by move=>X; right; rewrite mem_cat X Bool.orb_true_l.
+by move=> _ _; rewrite/btHasBlock dom_undef in_nil Bool.andb_false_l.
+Qed.
+
+Lemma btExtend_in_either bt b b' :
+  b ∈ btExtend bt b' -> b ∈ bt \/ b == b'.
+Proof.
+move=>X0; have X: (b ∈ (foldl btExtend bt [:: b'])) by [].
+case: (btExtend_fold_in_either X); first by left.
+by rewrite inE=>->; right.
+Qed.
+
+Lemma btExtend_fold_in bt xs b :
+  valid (foldl btExtend bt xs) -> b ∈ bt \/ b \in xs ->
+  b ∈ (foldl btExtend bt xs).
+Proof.
+elim/last_ind: xs=>[|xs x H]; first by move=>_; case=>//=.
+move=>V'; move: (btExtendV_fold1 V')=>V; specialize (H V).
+rewrite -cats1 foldl_cat //= {1}/btExtend.
+case: ifP; last first.
+- move=>D; case.
+  * move=>Hv; have X: (b ∈ bt \/ b \in xs) by left.
+    move: (H X); rewrite/btHasBlock=>/andP[] A B;
+    rewrite domPtUn inE validPtUn V D A Bool.orb_true_r //=;
+    (rewrite findPtUn2; last by rewrite validPtUn V D);
+    case: ifP=>//=; by move/eqP=>E; move: D A; rewrite E=>->.
+
+  * rewrite mem_cat inE=>/orP; case=>Hv.
+    have X: (b ∈ bt \/ b \in xs) by right.
+    move: (H X); rewrite/btHasBlock=>/andP[] A B;
+    rewrite domPtUn inE validPtUn V D A Bool.orb_true_r //=;
+    (rewrite findPtUn2; last by rewrite validPtUn V D);
+    case: ifP=>//=; by move/eqP=>E; move: D A; rewrite E=>->.
+
+  * by move/eqP in Hv; rewrite/btHasBlock domPtUn Hv inE eq_refl D;
+    rewrite validPtUn V D findPtUn ?validPtUn ?V ?D //=.
+case:ifP.
+* move=>F D; case=>Hv.
+  by (have X: (b ∈ bt \/ b \in xs) by left); move: (H X).
+  move: Hv; rewrite mem_cat inE=>/orP; case=>Hv.
+  by (have X: (b ∈ bt \/ b \in xs) by right); move: (H X).
+  by move/eqP in Hv; subst x; rewrite/btHasBlock D F.
+move=>F D; contradict V'.
+by rewrite -cats1 foldl_cat //= {1}/btExtend D F valid_undef.
+Qed.
+
+Lemma btExtend_idemp bt b :
+  valid (btExtend bt b) -> btExtend bt b = btExtend (btExtend bt b) b.
+Proof.
+move=>V'; move: (btExtendV V')=>V; rewrite{2}/btExtend; case: ifP.
+case: ifP=>//=.
+move=>X; rewrite{1}/btExtend; case: ifP=>D.
+case: ifP=>F; last by rewrite dom_undef.
+by move=>_; contradict X; rewrite/btExtend D F F.
+by contradict X; rewrite/btExtend D; rewrite findPtUn ?validPtUn ?V ?D //= eq_refl.
+move=>X; contradict X.
+rewrite/btExtend; case: ifP=>D.
+case: ifP=>F; first by rewrite D.
+by contradict V'; rewrite/btExtend D F valid_undef.
+by rewrite domPtUn inE validPtUn V D //= eq_refl.
+Qed.
+
+(* Just a reformulation *)
+Lemma btExtend_preserve (bt : BlockTree) ob b :
+  valid (btExtend bt b) ->
+  ob ∈ bt -> ob ∈ btExtend bt b.
+Proof.
+move=>V'; move: (btExtendV V')=>V; rewrite/btHasBlock=>/andP [H0 H1].
+rewrite/btExtend; case: ifP=>D.
+- case: ifP=>F.
+  by rewrite H0 H1.
+  by contradict V'; rewrite/btExtend D F valid_undef.
+have Vu: (valid (# b \\-> b \+ bt)) by rewrite validPtUn V D.
+rewrite findUnR // H0 H1 domUn inE Vu H0 /=.
+by apply/andP; split=>//=; apply/orP; right.
+Qed.
+
+Lemma btExtend_withDup_noEffect (bt : BlockTree) b:
+  b ∈ bt -> bt = (btExtend bt b).
+Proof. by rewrite/btHasBlock/btExtend=>/andP[]->->. Qed.
+
+(* There must be a better way to prove this. *)
+Lemma btExtend_comm bt b1 b2 :
+  valid (btExtend (btExtend bt b1) b2) ->
+  btExtend (btExtend bt b1) b2 = btExtend (btExtend bt b2) b1.
+Proof.
+move=>V2; move: (btExtendV V2)=>V1; move: (btExtendV V1)=>V0.
+have V1': valid (btExtend bt b2).
+rewrite/btExtend; case: ifP.
+- case: ifP=>//= F D.
+  contradict V2; rewrite{2}/btExtend; case: ifP.
+  case: ifP=>_ _; rewrite/btExtend.
+    by rewrite D F valid_undef.
+    by rewrite dom_undef validPtUn //= dom_undef valid_undef //=.
+  move=>Nd;
+  by rewrite/btExtend domPtUn validPtUn inE Nd V0 D Bool.orb_true_r //=;
+     rewrite findUnR ?validPtUn ?V0 ?Nd //= D F valid_undef.
+by move=>Nd; rewrite validPtUn V0 Nd.
+(* Now have V1' *)
+case A: (b1 ∈ bt).
+- move/andP: A=>[A0 A1].
+  rewrite ![btExtend _ b1]/btExtend A0 A1 (btExtend_dom V1' A0).
+  case: ifP=>//=; rewrite{1}/btExtend; case: ifP.
+  case: ifP; first by rewrite A1.
+  by move=>F D; contradict V1'; rewrite/btExtend D F valid_undef.
+  by move=>Nd; move: V1'; rewrite{1}/btExtend Nd=>V;
+     rewrite findUnR ?V1' //= A0 A1.
+case B: (b2 ∈ bt).
+- move/andP: B=>[B0 B1].
+  rewrite ![btExtend _ b2]/btExtend B0 (btExtend_dom V1 B0).
+  case: ifP; first by rewrite B1.
+  rewrite{1}/btExtend; move/nandP: A=>[A0|A1].
+  case: ifP; first by move=>D; rewrite D in A0.
+    by clear A0; move=>A0; rewrite findUnR ?validPtUn ?V0 ?A0 //= B0 B1.
+  rewrite B1; case: ifP.
+  case: ifP; first by move/eqP=>F; rewrite F in A1; move/eqP: A1.
+    by clear A1; move=>A1 A0 _; rewrite/btExtend A0 A1.
+   by move=>Nd; rewrite findUnR ?validPtUn ?V0 ?A0 ?Nd //= B0 B1.
+move/nandP: A=>[A0|A1]; move/nandP: B=>[B0|B1].
+- have VPt1: (forall a, valid (# b1 \\-> a \+ bt)). by move=>a; rewrite validPtUn V0 A0.
+  apply Bool.negb_true_iff in A0; apply Bool.negb_true_iff in B0.
+  rewrite/btExtend A0 B0; case: ifP.
+  + rewrite domPtUn VPt1 inE B0 //= =>/orP [] //==>/eqP H.
+    rewrite -H findUnR //= A0 domPtUn inE eq_refl VPt1 A0 findUnR //= A0 !findPt /=.
+    case: ifP; rewrite eq_sym=>/eqP; case: ifP=>/eqP=>//=.
+    by case=>->.
+  have VPt2: (forall a, valid (# b2 \\-> a \+ bt)). by move=>a; rewrite validPtUn V0 B0.
+  move=>X; have H: ((# b1 == # b2) = false)
+   by move: X; rewrite domPtUn inE VPt1 B0 //==>/norP [/eqP H _]; apply/eqP.
+  rewrite findUnR //= A0 domPtUn inE VPt2 A0 findPt2 eq_sym H //=.
+  by rewrite (joinC (#b1 \\-> _)) (joinC (#b2 \\-> _));
+    rewrite (joinC (#b2 \\-> _)) joinA (joinC bt).
+- have VPt1: (forall a, valid (# b1 \\-> a \+ bt)). by move=>a; rewrite validPtUn V0 A0.
+  apply Bool.negb_true_iff in A0;
+  rewrite/btExtend A0.
+  rewrite domPtUn VPt1 inE //=; case: ifP.
+  + move=>/orP [].
+    by move/eqP=>H; rewrite -H findUnR //= A0 findPt domUn VPt1 !inE domPt A0 inE eq_refl //=;
+       rewrite findUnR //= A0 findPt //= eq_sym; case: ifP=>//= /eqP[]->.
+    move=>D; rewrite findUnR //= D; case: ifP.
+      by move/eqP=>E; rewrite E in B1; move/eqP: B1.
+      by rewrite dom_undef //= join_undefR.
+  move/norP=>[Nh Nd]; case: ifP; case: ifP.
+  case: ifP; do? by move=>_ D; rewrite D in Nd.
+  by rewrite domPtUn inE A0=>Nd' /andP [] VPt2 /orP []=>//=;
+     move/eqP=>H; rewrite H in Nh; move/eqP: Nh.
+  by move=>D; rewrite D in Nd.
+  move=>_ _;
+  by rewrite (joinC (#b1 \\-> _)) (joinC (#b2 \\-> _));
+    rewrite (joinC (#b2 \\-> _)) joinA (joinC bt).
+- have VPt2: (forall a, valid (# b2 \\-> a \+ bt)). by move=>a; rewrite validPtUn V0 B0.
+  apply Bool.negb_true_iff in B0.
+  rewrite/btExtend B0 domPtUn VPt2 inE //=.
+  case: ifP; case: ifP; case: ifP;
+  do? by [
+    move/eqP=>A; rewrite A in A1; move/eqP: A1 |
+    rewrite dom_undef
+  ]. case: ifP.
+  move=>/orP [] //= /eqP H; rewrite H findUnL; last by rewrite -H; apply VPt2.
+  rewrite domPt inE eq_refl //= findUnR; last by rewrite -H; apply VPt2.
+  move=>F ->; rewrite findPt //=; case: ifP=>/eqP; first by case=>E; subst b2.
+  by move: F; rewrite findPt //= eq_sym=>/eqP.
+  by move/norP=>[]Nh _ F Nd;
+     rewrite domPtUn inE B0 //==>/andP [] _ /orP[]=>//= /eqP H;
+     rewrite H in Nh; move/eqP: Nh.
+  move=>X Y; rewrite domPtUn inE B0=>/andP [] _ /orP []=>//=/eqP H.
+  rewrite -H eq_refl //= findUnL; last by rewrite H; apply VPt2.
+  rewrite domPt inE eq_refl //= findPt //=; case: ifP=>//=.
+  move/eqP=>[E]; subst b2; contradict X.
+  by rewrite findUnR ?validPtUn ?V0 ?B0 //= findPt //==>/eqP.
+  move=>_ D; rewrite findUnR ?VPt2 //= D -(Bool.if_negb _ (find (# b1) bt == Some b1) _) A1.
+  case: ifP=>_ _; first by rewrite join_undefR.
+  have X: (# b1 \\-> b1 \+ bt = um_undef) by
+    apply invalidE; rewrite validPtUn V0 D.
+  by rewrite joinA (joinC (#b1 \\-> _)) -X joinA.
+  by move/orP=>[] //= /eqP H; rewrite H=>D; rewrite H in VPt2;
+     rewrite domPtUn inE D eq_refl VPt2.
+  by rewrite (joinC (#b1 \\-> _)) (joinC (#b2 \\-> _));
+    rewrite (joinC (#b2 \\-> _)) joinA (joinC bt).
+(* Nastiest case - 16 subcases to be handled one-by-one *)
+rewrite/btExtend; case: ifP; case: ifP; case: ifP; case: ifP.
+by move/eqP=>B; rewrite B in B1; move/eqP: B1.
+by move=>_ /eqP A; rewrite A in A1; move/eqP: A1.
+by rewrite dom_undef.
+by rewrite dom_undef.
+case: ifP; case: ifP.
+  by move/eqP=>B; rewrite B in B1; move/eqP: B1.
+  by rewrite dom_undef.
+  move=>_ D; rewrite domPtUn inE=>/andP[] _ /orP[].
+  by move/eqP=>H F Nd; move: F; rewrite H findUnL ?validPtUn ?V0 ?Nd //=;
+    rewrite domPt inE eq_refl findPt //==>/eqP[]->.
+  by move=>->.
+  move=>Nf Nd2 _ F Nd1. rewrite domPtUn inE Nd2 //==>/andP[]_ /orP[]=>//= /eqP H.
+  move: F; rewrite -H findUnL ?validPtUn ?V0 ?Nd1 //= domPt inE eq_refl //= findPt //=.
+  move/eqP=>[]E; subst b2; contradict Nf.
+  by rewrite findUnL ?validPtUn ?V0 ?Nd1 //= domPt inE eq_refl //= findPt //==>/eqP [].
+case: ifP.
+  case: ifP=>//=.
+  move=>_ D; contradict V1';
+  rewrite/btExtend D; case: ifP=>/eqP E;
+    by [rewrite E in B1; move/eqP: B1|rewrite valid_undef].
+  move=>D A F B; rewrite domPtUn inE D=>/andP []_/orP[] //= /eqP H; rewrite H.
+  by contradict A; rewrite domPtUn inE eq_sym H eq_refl D validPtUn V0 D.
+case: ifP; case: ifP=>//=.
+  by move/eqP=>B; rewrite B in B1; move/eqP: B1.
+  by rewrite dom_undef.
+  move=>F D _ Nf D'; move: F Nf; rewrite !findUnL ?validPtUn ?V0 ?D ?D' //=.
+  rewrite !domPt !inE //= inE (eq_sym (#b2)); case: ifP.
+  by move/eqP=>->; rewrite !findPt //==>/eqP []-> /eqP.
+  by move=>_ /eqP F; move: (find_some F)=>Nd'; rewrite Nd' in D'.
+case: ifP.
+  case: ifP; first by move/eqP=> B; move/eqP: B1; rewrite B.
+  by rewrite join_undefR.
+  move=>D _ _ _. rewrite domUn inE D domPt //= inE=>/andP []_/orP[]//=.
+  by move/eqP=><-; rewrite joinA pts_undef join_undefL.
+by move=>_/eqP A; rewrite A in A1; move/eqP: A1.
+by move=>_/eqP A; rewrite A in A1; move/eqP: A1.
+case: ifP; case: ifP.
+  by move/eqP=>B; rewrite B in B1; move/eqP: B1.
+  by rewrite dom_undef.
+  by move=>F D' _ _ D; move: F; rewrite findUnR ?validPtUn ?V0 ?D' //= D;
+     move/eqP=>A; rewrite A in A1; move/eqP: A1.
+  by rewrite join_undefR.
+case: ifP.
+  case: ifP; last by rewrite !join_undefR.
+  by move/eqP=> B; rewrite B in B1; move/eqP: B1.
+  rewrite join_undefR=>_ _ _ D _; rewrite joinA (joinC (#b1 \\-> _)).
+  suff: ~~ valid(#b1 \\-> b1 \+ bt) by move/invalidE; rewrite -joinA=>->; rewrite join_undefR.
+  by rewrite validPtUn V0 D.
+by case: ifP; [move=>_ _ -> | rewrite dom_undef].
+rewrite domPtUn inE=>_ /andP[]_/orP []; last by move=>->.
+  by move/eqP=>-> D; rewrite domPtUn inE eq_refl //= validPtUn V0 D.
+case: ifP.
+  by move/eqP=>B; rewrite B in B1; move/eqP: B1.
+  by move=>_D D' _; rewrite domPtUn validPtUn V0 inE D' //==>-> //= /norP[].
+by move=>_ _ _ _; rewrite !joinA (joinC (#b2 \\-> _)).
+Qed.
+
+Definition no_collisions (bt : BlockTree) (xs : seq BType) :=
+  valid bt /\
+  forall a, a \in xs ->
+    (forall b, b \in xs -> # a = # b -> a = b) /\
+    (forall b, b ∈ bt -> # a = # b -> a = b).
+
+Lemma btExtendV_valid_no_collisions bt xs :
+  valid (foldl btExtend bt xs) -> no_collisions bt xs.
+Proof.
+elim/last_ind: xs=>[|xs x H0] //=.
+- move=>V; move: (btExtendV_fold1 V)=>V1; specialize (H0 V1).
+  move: H0; rewrite/no_collisions.
+  move=>[] V0 N; split=>//=.
+  move=>a; rewrite -cats1 mem_cat inE=>/orP; case; last first.
+  * move/eqP=>E; subst a; split.
+    move=>b; rewrite mem_cat inE=>/orP; case; last first.
+    by rewrite eq_sym=>/eqP.
+    by apply (btExtendV_fold_dup V).
+    move=>b; rewrite/btHasBlock=>/andP[D F] Hh.
+    move: V; rewrite -cats1 foldl_cat //= {1}/btExtend.
+    move: (btExtend_dom_fold V1 D)=>D'; rewrite Hh D'.
+    case: ifP; last by rewrite valid_undef.
+    move=>F' _; move/eqP in F'.
+    by move: (btExtend_find_fold V1 D F'); move/eqP: F=>-> []->.
+  move=>X; specialize (N a X); case: N=>N0 N1; split=>b; last by apply N1.
+  rewrite mem_cat inE=>/orP; case; first by apply N0.
+  move/eqP=>E; subst b=>/eqP Hh; rewrite eq_sym in Hh; move/eqP in Hh.
+  by move: (btExtendV_fold_dup V X Hh)=>->.
+Qed.
+
+Lemma btExtendV_no_collisions_valid bt xs :
+  validH bt -> no_collisions bt xs -> valid (foldl btExtend bt xs).
+Proof.
+elim/last_ind: xs=>[|xs x H1] //=.
+by rewrite/no_collisions=>_; case.
+rewrite/no_collisions=>Vh; case=>V N.
+have N0: no_collisions bt xs.
+rewrite/no_collisions; split=>//=.
+  move=>a X; have X0: a \in rcons xs x
+    by rewrite mem_rcons inE X Bool.orb_true_r.
+  specialize (N a X0); move: N=>[]N0 N1; split=>b; last by apply N1.
+  move=>X1; have X2: b \in rcons xs x.
+    by rewrite mem_rcons inE X1 Bool.orb_true_r.
+  by apply N0.
+specialize (H1 Vh N0); rewrite -cats1 foldl_cat //= {1}/btExtend.
+case: ifP; last by move=>D; rewrite validPtUn H1 D.
+case: ifP=>//= F D; contradict H1.
+(* Hmm *)
+have X: (x \in rcons xs x) by rewrite mem_rcons mem_head.
+specialize (N x X); move: N0=>N'; case: N=>N0 N1.
+move: (um_eta D)=>[b] [F'] zz; rewrite F' in F.
+specialize (N0 b); specialize (N1 b).
+move: (btExtendH_fold Vh (dom_valid D) F')=>Hh.
+rewrite Hh in D F'; have H: b ∈ (foldl btExtend bt xs).
+  by rewrite/btHasBlock D F' eq_refl.
+case Z: (x == b); first by move/eqP: Z F=>->; rewrite eq_refl.
+case: (btExtend_fold_in_either H).
+by move=>Q; move: (N1 Q Hh) Z=>->; rewrite eq_refl.
+move=>R; have Q: (b \in rcons xs x)
+  by rewrite -cats1 mem_cat inE R Bool.orb_true_l.
+by move: (N0 Q Hh) Z=>->; rewrite eq_refl.
+Qed.
+
+Lemma btExtendV_fold_comm' bt xs ys :
+  validH bt ->
+  valid (foldl btExtend (foldl btExtend bt xs) ys) ->
+  valid (foldl btExtend (foldl btExtend bt ys) xs).
+Proof.
+move=>Vh.
+elim/last_ind: ys=>[|ys y V1]//= V.
+move: (btExtendV_fold1 V)=>V0; specialize (V1 V0).
+rewrite -foldl_cat; apply btExtendV_no_collisions_valid=>//=.
+rewrite/no_collisions; split.
+have X: (xs = [::] ++ xs) by [].
+by move: V0; rewrite -foldl_cat X; move/btExtendV_fold/btExtendV_fold.
+move: V; rewrite -foldl_cat; move/btExtendV_valid_no_collisions.
+rewrite/no_collisions; case=>V H.
+move=>a; rewrite mem_cat Bool.orb_comm=>X.
+specialize (H a); rewrite mem_cat in H; specialize (H X).
+case: H=>H0 H1; split=>//=.
+move=>b; rewrite mem_cat Bool.orb_comm -mem_cat; apply H0.
+Qed.
+
+Lemma btExtendV_fold_comm bt xs ys :
+  validH bt ->
+  valid (foldl btExtend (foldl btExtend bt xs) ys) =
+  valid (foldl btExtend (foldl btExtend bt ys) xs).
+Proof.
+move=>Vh.
+have T: true by [].
+have X: forall (a b : bool), a <-> b -> a = b.
+by move=>a b []; case: a; case: b=>//= A B;
+   [specialize (A T) | specialize (B T)].
+by apply X; split; apply btExtendV_fold_comm'.
+Qed.
+
+Lemma btExtendV_fold' bt xs ys :
+  validH bt-> valid (foldl btExtend bt (xs ++ ys)) -> valid (foldl btExtend bt ys).
+Proof. by move=>Vh; rewrite foldl_cat btExtendV_fold_comm //= -foldl_cat=>/btExtendV_fold. Qed.
 
 End Forests.
