Structures/ConsensusState.v
@@ -1,0 +1,837 @@
+From mathcomp.ssreflect
+Require Import ssreflect ssrbool ssrnat eqtype ssrfun seq fintype path.
+Require Import Eqdep.
+From fcsl
+Require Import pred prelude ordtype pcm finmap unionmap heap.
+From LibraChain
+Require Import SeqFacts Chains HashSign Blocks.
+Set Implicit Arguments.
+Unset Strict Implicit.
+Unset Printing Implicit Defensive.
+
+(* A formalization of a block forests *)
+
+(************************************************************)
+(******************* <parameters> ***************************)
+(************************************************************)
+Section State.
+
+Variable Hash : ordType.
+Variables (PublicKey: Type) (Signature: eqType) (Address: hashType PublicKey).
+
+Parameters (Command NodeTime: Type).
+
+(* The Block Data (w/o signatures) *)
+Notation BDataType := (BlockData Hash Signature Address Command NodeTime).
+
+Variable hashB: BDataType -> Hash.
+Hypothesis inj_hashB: injective hashB.
+
+Variable verifB: Hash -> PublicKey -> Signature -> bool.
+
+(* Block Type : block data with signatures *)
+Notation BType := (BlockType inj_hashB verifB).
+Notation QC := (QuorumCert Hash Signature (Phant Address)).
+
+Implicit Type b: BType.
+
+Parameter GenesisBlock : BType.
+
+Definition genesis_round := (round (block_data GenesisBlock)).
+
+Definition qc_of b := (proof (block_data b)).
+
+(************************************************************)
+(** Consensus State                                        **)
+(************************************************************)
+
+Record ConsensusState := mkConsensusState {
+  last_vote_round: nat;
+  preferred_block_round: nat;
+}.
+
+Definition consensusstate2nats (cs: ConsensusState) :=
+  let: mkConsensusState lvr pvr := cs in (lvr, pvr).
+
+Definition nats2consensusstate (nats: nat * nat) :=
+  let: (lvr, pbr) := nats in mkConsensusState lvr pbr.
+
+Lemma can_cs_nats: ssrfun.cancel consensusstate2nats nats2consensusstate.
+Proof. by move => []. Qed.
+
+Definition cs_eqMixin := CanEqMixin can_cs_nats.
+Canonical cs_eqType := EqType _ cs_eqMixin.
+
+Definition genesis_state := mkConsensusState genesis_round genesis_round.
+
+Implicit Type state: ConsensusState.
+
+Definition update state (qc: QC) :=
+  let: round := (block_round (qc_vote_data qc)) in
+  if (round > preferred_block_round state) then
+    mkConsensusState (last_vote_round state) (round)
+  else
+    state.
+
+Lemma update_eq_lvr state qc :
+  last_vote_round (update state qc) = last_vote_round state.
+Proof.
+rewrite /update.
+by case (block_round (qc_vote_data qc) > preferred_block_round state).
+Qed.
+
+Lemma update_pbr_geq state qc :
+  preferred_block_round state <= preferred_block_round (update state qc).
+Proof.
+rewrite /update.
+case H: (block_round (qc_vote_data qc) > preferred_block_round state) => //.
+by move/ltnW: H => ->.
+Qed.
+
+Lemma update_qc_gt state qc :
+  block_round (qc_vote_data qc) <= preferred_block_round (update state qc).
+Proof.
+rewrite /update; case H: (preferred_block_round state < (block_round (qc_vote_data qc))) => //.
+by rewrite leqNgt H.
+Qed.
+
+Lemma update_pbr_P state qc:
+  reflect (preferred_block_round (update state qc) = block_round (qc_vote_data qc))
+          (preferred_block_round state <= block_round (qc_vote_data qc)).
+Proof.
+apply: (iffP idP); rewrite /update;
+case H: (block_round (qc_vote_data qc) > preferred_block_round state);
+rewrite leq_eqVlt H ?orbF ?orbT //; move/eqP=> //.
+Qed.
+
+Lemma update_maxn state qc:
+  update state qc =
+  mkConsensusState (last_vote_round state)
+                   (maxn (preferred_block_round state) (block_round (qc_vote_data qc))).
+Proof.
+rewrite /update /maxn; case: ((preferred_block_round state) < (block_round (qc_vote_data qc))) => //=.
+by case state.
+Qed.
+
+(************************************************************)
+(** Voting after update with the QC                        **)
+(************************************************************)
+
+Definition votable state b :=
+  let: (rd, lvr, pbr) :=
+     ((round b),
+     (last_vote_round state),
+     (preferred_block_round state)) in [&& rd > lvr & rd >= pbr].
+
+Lemma votable_updateP state b:
+  reflect (votable (update state (qc_of b)) b)
+  (votable state b && (round b >= block_round (qc_vote_data (qc_of b)))).
+Proof.
+  apply: (iffP andP); rewrite /votable update_eq_lvr.
+- rewrite /update; case (preferred_block_round state < block_round (qc_vote_data (qc_of b)));
+  by move=> [H1 H2]; move/andP: H1=> [-> H1] //; rewrite ltnW //.
+- move/andP => [->] //= H.
+  apply/andP; rewrite (leq_trans (update_pbr_geq _ _) H) //=.
+  by apply: (leq_trans (update_qc_gt state _)).
+Qed.
+
+Lemma votable_update_round_geq state b:
+  (votable (update state (qc_of b)) b) =
+  (votable state b && (round b >= block_round (qc_vote_data (qc_of b)))).
+Proof.
+by apply/(sameP idP); apply: votable_updateP.
+Qed.
+
+Definition voting_rule state (b: BType) :=
+  let after_update := update state (qc_of b) in
+  if votable (after_update) b then
+    let newState :=
+        mkConsensusState (round b) (preferred_block_round after_update)
+    in
+    (newState, true)
+  else (after_update, false).
+
+Definition voted_on state b := (voting_rule state b).2.
+
+Lemma voted_on_votable state b:
+  voted_on state b = votable (update state (qc_of b)) b.
+Proof.
+rewrite /voted_on /voting_rule.
+by case: (votable (update state (qc_of b)) b) => //.
+Qed.
+
+Lemma voted_br_gt_qcr state b:
+  voted_on state b = true ->
+  round b >= block_round (qc_vote_data (qc_of b)).
+Proof.
+rewrite /voted_on /voting_rule.
+case H: (votable (update state (qc_of b)) b).
+- by move/votable_updateP: H; move/andP => [_ ->].
+- by rewrite /update; case (preferred_block_round state < _).
+Qed.
+
+Lemma ineq_voted_on state b:
+  (voted_on state b) = [&& (round b > last_vote_round state),
+                         (round b >= preferred_block_round state) &
+                         (round b >= block_round (qc_vote_data (qc_of b)))].
+Proof.
+by rewrite voted_on_votable votable_update_round_geq /votable -andbA.
+Qed.
+
+
+Lemma vote_genesis_N: voted_on genesis_state GenesisBlock = false.
+Proof.
+by rewrite voted_on_votable /votable update_eq_lvr /= /genesis_round ltnn.
+Qed.
+
+Definition next_state state b := (voting_rule state b).1.
+
+Lemma next_state_pbr_update state b :
+  preferred_block_round (next_state state b) = preferred_block_round (update state (qc_of b)).
+Proof.
+by rewrite /next_state /voting_rule; case (votable (update state (qc_of b)) b).
+Qed.
+
+Lemma next_state_pbr_geq state b:
+  preferred_block_round state <= preferred_block_round (next_state state b).
+Proof.
+by rewrite next_state_pbr_update update_pbr_geq.
+Qed.
+
+Lemma next_state_lvr_voted state b :
+  reflect (last_vote_round state < last_vote_round (next_state state b)) (voted_on state b).
+Proof.
+rewrite /next_state /voting_rule -voted_on_votable; apply: (iffP idP).
+- move=>H; rewrite (H)=>//=; move:H; rewrite ineq_voted_on.
+  by move/andP=>[-> _].
+- by case: (voted_on state b); rewrite // update_eq_lvr ltnn.
+Qed.
+
+Lemma next_state_lvr_round state b:
+  voted_on state b -> last_vote_round (next_state state b) = round b.
+Proof.
+by rewrite voted_on_votable /next_state /voting_rule=>-> /=.
+Qed.
+
+Lemma next_state_lvr_static state b:
+  ~~ voted_on state b -> last_vote_round (next_state state b) = last_vote_round state.
+Proof.
+rewrite voted_on_votable /next_state /voting_rule.
+by move/negbTE=>->; rewrite update_eq_lvr.
+Qed.
+
+
+Lemma next_state_lvr_if state b:
+  next_state state b =
+  let: pbr:= preferred_block_round (update state (qc_of b)) in
+     if (voted_on state b) then
+       mkConsensusState (round b) pbr
+     else
+       mkConsensusState (last_vote_round state) pbr.
+Proof.
+rewrite /next_state /voting_rule -voted_on_votable /=; case H: (voted_on state b)=> //=.
+by rewrite update_maxn /=.
+Qed.
+
+Lemma next_state_lvr_leq state b:
+  last_vote_round state <= last_vote_round (next_state state b).
+Proof.
+case H: (voted_on state b).
+- by rewrite leq_eqVlt; move/next_state_lvr_voted: H=>->; rewrite orbT.
+- by rewrite /next_state /voting_rule -voted_on_votable H update_eq_lvr.
+Qed.
+
+Lemma next_state_maxn state b:
+  (next_state state b) =
+  let: u_pbr := (maxn (preferred_block_round state) (block_round (qc_vote_data (qc_of b)))) in
+  mkConsensusState
+    (if (round b) >= maxn ((last_vote_round state).+1) u_pbr then round b else last_vote_round state)
+    u_pbr.
+Proof.
+rewrite /next_state /voting_rule update_maxn.
+set pbr:= (maxn (preferred_block_round state) (block_round (qc_vote_data (qc_of b)))).
+rewrite /votable /= -geq_max.
+by case H: (maxn (last_vote_round state).+1 pbr <= round b).
+Qed.
+
+Lemma pbr_next_stateC state b c:
+  preferred_block_round (next_state (next_state state b) c) =
+  preferred_block_round (next_state (next_state state c) b).
+Proof.
+rewrite (next_state_maxn (next_state state c) b) next_state_maxn /=.
+by rewrite !next_state_maxn /= maxnAC.
+Qed.
+
+Lemma voting_next_voted state b :
+  voting_rule state b = (next_state state b, voted_on state b).
+Proof.
+by apply surjective_pairing.
+Qed.
+
+Lemma voting_next_N state b: voted_on (next_state state b) b = false.
+Proof.
+rewrite voted_on_votable votable_update_round_geq /votable.
+rewrite {1}/next_state /voting_rule.
+case H:(votable (update state (qc_of b)) b) => /=; first by rewrite ltnn.
+rewrite /votable -next_state_pbr_update in H.
+by rewrite H andFb.
+Qed.
+
+Lemma voting_update_progress state qc x:
+  voted_on (update state qc) x -> voted_on state x.
+Proof.
+rewrite 2!ineq_voted_on update_maxn /= geq_max.
+by move/andP=>[->]; move/andP =>[H ->]; move/andP: H=>[-> _].
+Qed.
+
+Lemma voting_progress state b x:
+  voted_on (next_state state b) x -> voted_on state x.
+Proof.
+rewrite 2!ineq_voted_on; move/andP=> [Hlvr]; move/andP=> [Hpbr Hbr].
+rewrite (leq_ltn_trans (next_state_lvr_leq _ _) Hlvr).
+by rewrite (leq_trans (next_state_pbr_geq _ _) Hpbr) /=.
+Qed.
+
+Lemma voting_gt state b x:
+  voted_on (next_state state b) x ->
+  ~~ voted_on state b || (round b < round x).
+Proof.
+move=> H; move: (H); rewrite ineq_voted_on; move/andP=> [Hlvr _].
+case I: (voted_on state b)=> //.
+by rewrite (next_state_lvr_round I) in Hlvr.
+Qed.
+
+Lemma non_voted_on_update state b x:
+  ~~ voted_on state b ->
+  voted_on (next_state state b) x = voted_on (update state (qc_of b)) x.
+Proof.
+rewrite next_state_lvr_if; move/negbTE=>->.
+by rewrite update_maxn.
+Qed.
+
+Lemma pbr_update_next state b x:
+  preferred_block_round (update (next_state state b) (qc_of x)) =
+  preferred_block_round (update (update state (qc_of b)) (qc_of x)).
+Proof.
+by rewrite next_state_maxn !update_maxn /=.
+Qed.
+
+Lemma voted_next_update state b x:
+  voted_on (next_state state b) x ->
+  voted_on (update state (qc_of b)) x.
+Proof.
+move=> H; move/voting_progress: (H); rewrite ineq_voted_on; move/andP=> [Hs _].
+move: H; rewrite ineq_voted_on next_state_pbr_update.
+move/andP=>[Hlvr]; move/andP=> [H1 H2].
+by rewrite ineq_voted_on update_eq_lvr Hs H1 H2.
+Qed.
+
+(* TODO: figure out if we want to keep this one, probably obsoleted by *)
+(* comparator reasoning?*)
+Lemma next_stateC state b c:
+  next_state (next_state state b) c =
+  if (~~ voted_on state b || ((round b < round c) &&
+     (block_round (qc_vote_data (qc_of c)) <= round c))) then
+    next_state (update state (qc_of b)) c
+  else
+    (update (next_state state b) (qc_of c)).
+Proof.
+rewrite next_state_lvr_if [next_state (update _ _)_]next_state_lvr_if .
+case H: (~~ voted_on state b).
+- move/idP: (H); move/non_voted_on_update=> ->.
+  by rewrite pbr_update_next (next_state_lvr_static H) update_eq_lvr.
+move/negPn: H=> H; case I: (voted_on (next_state state b) c).
+- move/idP: (I); move/voting_gt; rewrite H /= ltnNge; move/negbTE =>->.
+  move/idP: (I); move/voted_next_update=>->; rewrite pbr_update_next /=.
+  by move/idP: I; move/voting_progress; move/voted_br_gt_qcr=>->.
+move/negbT: (I); rewrite ineq_voted_on negb_and.
+rewrite (next_state_lvr_round H) next_state_pbr_update.
+rewrite ineq_voted_on; move/orP=>[|].
+- by move/negbTE=>->/=; rewrite update_maxn (next_state_lvr_round H) /=.
+move/negbTE=>->; rewrite andbF orFb update_eq_lvr pbr_update_next.
+case J: (round b < round c);
+last by rewrite !update_maxn (next_state_lvr_round H) next_state_pbr_update !update_maxn /=.
+move/negbT: (I); rewrite voted_on_votable /votable.
+move: (H); rewrite ineq_voted_on; move/andP=> [Hlvr]; move/andP=> [Hpbr Hbr].
+rewrite update_maxn (next_state_lvr_round H) J andTb; move/idP: J=> J/=.
+rewrite next_state_maxn /= maxnAC geq_max.
+rewrite [block_round (qc_vote_data (qc_of b)) <= _]leq_eqVlt (leq_ltn_trans Hbr J) orbT andbT.
+rewrite geq_max leq_eqVlt (leq_ltn_trans Hpbr J) orbT andTb; move/negbTE=>-> /=.
+by rewrite !update_maxn /= maxnAC.
+Qed.
+
+Lemma next_state_updateC state qc x:
+  voted_on (update state qc) x ->
+  next_state (update state (qc)) x =
+  update (next_state state x) qc.
+Proof.
+move => H; rewrite /next_state /voting_rule -2!voted_on_votable H.
+by move/voting_update_progress: H=> -> /=; rewrite !update_maxn /= maxnAC.
+Qed.
+
+Lemma voted_on_maxn state b:
+  (voted_on state b) =
+  (round b >= maxn
+               (maxn ((last_vote_round state).+1) (preferred_block_round state))
+               (block_round (qc_vote_data (qc_of b)))).
+Proof.
+by rewrite !geq_max -andbA ineq_voted_on.
+Qed.
+
+(************************************************************)
+(** Voting in Sequence                                     **)
+(************************************************************)
+
+Implicit Type bseq: seq BType.
+
+(* node_processing is a slight modification on a scanleft of the voting rules
+over a seq of block *)
+Fixpoint process_aux state bseq res :=
+  if bseq is x::s then
+    let: (new_state, vote) := (voting_rule state x) in
+    process_aux new_state s ((state, vote) :: res)
+  else
+    (state, rev res).
+
+Definition node_processing state bseq := process_aux state bseq [::].
+
+Lemma size_process_aux state bseq res: size (process_aux state bseq res).2 = size bseq + size res.
+Proof.
+elim:bseq res state => [|x xs IHs] res state.
+- by rewrite size_rev add0n.
+- by rewrite /= voting_next_voted IHs /= addSnnS.
+Qed.
+
+Lemma size_processing state bseq : size (node_processing state bseq).2 = size bseq.
+Proof.
+by rewrite /node_processing size_process_aux addn0.
+Qed.
+
+Lemma processing_aux_state_res_irrel state bseq rs1 rs2:
+  (process_aux state bseq rs1).1 = (process_aux state bseq rs2).1.
+Proof.
+elim: bseq state rs1 rs2 => [|b bs IHb] state rs1 rs2 //=; rewrite voting_next_voted.
+by apply:IHb.
+Qed.
+
+Lemma processing_aux_rcons state bseq r rs:
+  (process_aux state bseq (rcons rs r)).2 =
+  r :: (process_aux state bseq rs).2.
+Proof.
+elim: bseq r rs state =>[| b bs IHb] r rs state => /=.
+- by rewrite rev_rcons.
+- by rewrite voting_next_voted -IHb -rcons_cons.
+Qed.
+
+Lemma processing_aux_rev state bseq res:
+  (process_aux state bseq res).2 =
+  rev res ++ (process_aux state bseq [::]).2.
+Proof.
+move: res bseq state; apply: last_ind=> [|rs r IHr] bseq state.
+- by [].
+- by rewrite processing_aux_rcons IHr rev_rcons.
+Qed.
+
+Lemma processing_aux_cons state b bs:
+  (process_aux state (b::bs) [::]).2 =
+  (state, voted_on state b) :: (process_aux (next_state state b) bs [::]).2.
+Proof.
+rewrite /= voting_next_voted -[[:: (state, voted_on _ _)]]cat0s cats1.
+by rewrite processing_aux_rcons.
+Qed.
+
+Lemma processing_aux_cons2 state b bs:
+  (process_aux state (b::bs) [::]) =
+  let: (f_state, vbs) := (process_aux (next_state state b) bs [::]) in
+  (f_state, (state, voted_on state b) ::vbs).
+Proof.
+rewrite /= voting_next_voted -[[:: (state, voted_on _ _)]]cat0s cats1.
+rewrite [process_aux _ bs [::]]surjective_pairing -processing_aux_cons /=.
+rewrite (processing_aux_state_res_irrel _ _ [::] [:: (state, voted_on state b)]).
+by rewrite voting_next_voted -surjective_pairing.
+Qed.
+
+Lemma node_processing_cons state b bs:
+  (node_processing state (b::bs)).2 =
+  (state, voted_on state b) :: (node_processing (next_state state b) bs).2.
+Proof.
+by rewrite processing_aux_cons.
+Qed.
+
+Lemma node_processing_cons2 state b bs:
+  (node_processing state (b::bs)) =
+  let: (final_state, bsvotes) := node_processing (next_state state b) bs in
+  (final_state, (state, voted_on state b)::bsvotes).
+Proof.
+by  rewrite /node_processing processing_aux_cons2.
+Qed.
+
+Lemma node_processing_cons1 state b bs:
+  (node_processing state (b::bs)).1 =
+  (node_processing (next_state state b) bs).1.
+Proof.
+case: bs state b=>[|x s ]=>state b; rewrite node_processing_cons2 //=.
+by rewrite [node_processing _ _]surjective_pairing /=.
+Qed.
+
+Lemma node_processing_cat_cps state bs1 bs2 :
+  (node_processing state (bs1 ++ bs2)) =
+  let: (state1, seq1) := (node_processing state bs1) in
+  let: (state2, seq2) := (node_processing state1 bs2) in
+  (state2, seq1 ++ seq2).
+Proof.
+elim: bs1 state =>[| b bs IHb] state /=.
+- by rewrite {2}[node_processing _ _]surjective_pairing -surjective_pairing.
+rewrite 2!node_processing_cons2 IHb [node_processing (next_state _ _) _]surjective_pairing /=.
+by rewrite [node_processing _  _]surjective_pairing.
+Qed.
+
+Lemma node_processing_rcons state bs b:
+  (next_state (node_processing state bs).1 b) =
+  (node_processing state (rcons bs b)).1.
+Proof.
+rewrite -cats1 node_processing_cat_cps /=.
+rewrite {2}[node_processing _ _]surjective_pairing /=.
+rewrite [node_processing _ [::b]]surjective_pairing /=.
+by rewrite node_processing_cons1 /=.
+Qed.
+
+Lemma voting_progress_seq state bs b:
+  voted_on (node_processing state bs).1 b -> voted_on state b.
+Proof.
+elim: bs state b => [|x s IHs] state b //=.
+rewrite node_processing_cons1.
+move/IHs; apply voting_progress.
+Qed.
+
+(************************************************************)
+(** Consensus State Comparators                            **)
+(************************************************************)
+
+Definition comparator state1 :=
+  maxn (last_vote_round state1).+1 (preferred_block_round state1).
+
+Definition state_compare state1 state2 :=
+  comparator state1 <= comparator state2.
+
+Delimit Scope state_scope with STATE.
+Open Scope state_scope.
+
+Notation "state1 <% state2" := (state_compare state1 state2) (at level 40) :state_scope.
+
+Lemma voting_comparator state x:
+  (voted_on state x) ->
+  (comparator (next_state state x) = (round x).+1).
+Proof.
+rewrite next_state_lvr_if fun_if /comparator /= =>H.
+rewrite H; apply/maxn_idPl; move/idP:H; rewrite voted_on_votable.
+by move/andP=>[_ H]; apply ltnW; rewrite ltnS.
+Qed.
+
+Lemma non_voting_comparator state x:
+  ~~ voted_on state x ->
+  comparator (next_state state x) = maxn (comparator state) (block_round (qc_vote_data (qc_of x))).
+Proof.
+move=>Hnv; rewrite next_state_lvr_if; move/negbTE: (Hnv)=>->.
+by rewrite /comparator update_maxn /= maxnA.
+Qed.
+
+Lemma voting_comparator_eq state b:
+    (voted_on state b) =
+    ((comparator state <= round b) && (block_round (qc_vote_data (qc_of b)) <= round b))
+    .
+Proof.
+by rewrite /comparator geq_max -andbA -ineq_voted_on.
+Qed.
+
+Lemma voting_gt_compare state1 state2 x:
+  state1 <% state2 -> voted_on state2 x -> voted_on state1 x.
+Proof.
+move=> H; rewrite 2!voted_on_maxn; apply leq_trans.
+rewrite geq_max leq_maxr leq_max andbT.
+by apply/orP; left.
+Qed.
+
+Lemma voting_next_gt state x:
+  state <% (next_state state x).
+Proof.
+rewrite next_state_lvr_if.
+case Hx:(voted_on state x); rewrite /state_compare /=.
+- move/idP: Hx; rewrite voted_on_maxn.
+  rewrite leq_max geq_max; move/andP=> [H _].
+  by apply/orP; left; apply ltnW.
+rewrite update_maxn /= leq_max 2!geq_max ltnS leqnn andTb.
+rewrite leq_maxl andbT leq_max.
+case I: (last_vote_round state < preferred_block_round state);
+first by rewrite orTb orbT.
+move/negbT: I; rewrite ltnNge; move/negPn=> H.
+by rewrite orFb; apply/orP; left; apply ltnW.
+Qed.
+
+Lemma voting_processing_gt state bs:
+  state <% (node_processing state bs).1.
+Proof.
+elim: bs state=> [|b s IHs] state /=; first by rewrite /state_compare.
+rewrite node_processing_cons1; move:(@voting_next_gt state b).
+move/leq_trans; apply; apply IHs.
+Qed.
+
+Lemma voting_next_inner state1 state2 x:
+  state1 <% state2 ->
+  (next_state state1 x) <% (next_state state2 x).
+Proof.
+move => H12.
+case H2: (voted_on state2 x).
+- rewrite /state_compare (voting_comparator H2).
+  move/(voting_gt_compare H12): H2; move/voting_comparator=>->.
+  by apply: ltnSn.
+case H1: (voted_on state1 x).
+- rewrite /state_compare (voting_comparator H1).
+  rewrite /comparator; move/negbT: (H2); rewrite voted_on_votable.
+  rewrite /votable /= next_state_pbr_update next_state_lvr_if H2 /=.
+  rewrite negb_and -leqNgt -ltnNge leq_max.
+  move/orP=>[|->]; last by rewrite orbT.
+  by rewrite update_maxn /= ltnS =>->.
+rewrite 2!next_state_lvr_if H1 H2.
+move: H12; rewrite /state_compare /comparator 2!update_maxn /=.
+rewrite !maxnA=>H12; rewrite geq_max leq_max H12 orTb andTb.
+by rewrite leq_max leqnn orbT.
+Qed.
+
+Lemma voting_processing_inner state1 state2 bs:
+  state1 <% state2 ->
+  (node_processing state1 bs).1 <% (node_processing state2 bs).1.
+Proof.
+move: state1 state2; elim bs => [|b s IHs]=> state1 state2 H12 //.
+by rewrite 2!node_processing_cons1 IHs // voting_next_inner.
+Qed.
+
+(************************************************************)
+(** Sequence of elements which a node voted on             **)
+(************************************************************)
+
+Definition voted_in_processing state bseq :=
+  mask (unzip2 (node_processing state bseq).2) bseq.
+
+Lemma voted_in_processing_cat_cps state bs1 bs2:
+  (voted_in_processing state (bs1 ++ bs2)) =
+  let: b1 := (voted_in_processing state bs1) in
+  let: b2 := (voted_in_processing (node_processing state bs1).1 bs2) in
+  b1 ++ b2.
+Proof.
+rewrite /voted_in_processing node_processing_cat_cps /=.
+rewrite 2![node_processing _ _]surjective_pairing /=.
+rewrite -mask_cat; last by rewrite size_map size_processing.
+by rewrite -map_cat /unzip2.
+Qed.
+
+Lemma voted_in_processing_cons state b bs:
+  (voted_in_processing state (b::bs)) =
+  (nseq (voted_on state b) b ++ (voted_in_processing (next_state state b) bs)).
+Proof.
+by rewrite /voted_in_processing node_processing_cons mask_cons.
+Qed.
+
+Lemma comparatorC state b c:
+  comparator (next_state (next_state state b) c) =
+  comparator (next_state (next_state state c) b).
+Proof.
+rewrite next_state_maxn maxnA -/(comparator (next_state _ _)).
+rewrite [next_state (next_state _ _) _]next_state_maxn maxnA.
+rewrite -/(comparator (next_state _ _)) 2!geq_max 2!next_state_pbr_update 2!update_maxn /=.
+rewrite 2![comparator {|last_vote_round := _; preferred_block_round:= _|}]/comparator /= maxnAC.
+case Hc: (voted_on state c); [rewrite (next_state_lvr_round Hc) (voting_comparator Hc) (voted_br_gt_qcr Hc) andbT
+  | move/negbT/next_state_lvr_static: (Hc)=>->; rewrite (non_voting_comparator (negbT Hc)) geq_max];
+case Hb: (voted_on state b); [ rewrite (next_state_lvr_round Hb) (voting_comparator Hb) (voted_br_gt_qcr Hb) andbT
+  | move/negbT/next_state_lvr_static: (Hb)=>->; rewrite (non_voting_comparator (negbT Hb)) geq_max
+  | rewrite (next_state_lvr_round Hb) (voting_comparator Hb) (voted_br_gt_qcr Hb) andbT
+  | move/negbT/next_state_lvr_static: (Hb)=>->; rewrite (non_voting_comparator (negbT Hb)) geq_max].
+- case Hbc: (round b == round c); first by move/eqP: Hbc; move=><-; rewrite ltnn.
+  by move/negbT: (Hbc); rewrite neq_ltn; move/orP=>[Hltn|Hltn]; rewrite Hltn /=; move: Hltn; rewrite ltnNge leq_eqVlt;
+  [rewrite eq_sym|]; rewrite Hbc orFb; move/negbTE=>->/=.
+- move: (Hc); rewrite voting_comparator_eq; move/andP=>[Hcpc Hbrc] /=.
+  rewrite Hcpc; move/negbT: (Hb); rewrite voting_comparator_eq negb_and.
+  case Hbrb: ((block_round (qc_vote_data (qc_of b))) <= round b); [rewrite orbF andbT andTb -ltnNge => Hcpb | rewrite andbF andTb => _ ].
+  - by rewrite ltnNge; move/ltnW: (leq_trans Hcpb Hcpc)=> Hbc; rewrite Hbc (leq_trans Hbrb Hbc) /=.
+  move/negbT: Hbrb; rewrite -ltnNge=> Hbrb; case Hqbc: (block_round (qc_vote_data (qc_of b)) <= round c); first by [].
+  move/negbT: Hqbc; rewrite -ltnNge=> Hqbc; rewrite [maxn (round c).+1 _]maxnCA; move/maxn_idPr: (Hqbc)=>->.
+  rewrite 2!maxnA -/(comparator state) maxnAC; move/ltnW: (leq_ltn_trans Hcpc Hqbc); move/maxn_idPr=>->.
+  move: (leq_maxr (last_vote_round state).+1 (preferred_block_round state)); rewrite -/(comparator state)=> Hprcsc.
+  by rewrite maxnAC; move: (leq_ltn_trans (leq_trans Hprcsc Hcpc) Hqbc); move/ltnW/maxn_idPr=>->.
+- move: (Hb); rewrite voting_comparator_eq; move/andP=>[Hcpb Hbrb] /=.
+  rewrite Hcpb; move/negbT: (Hc); rewrite voting_comparator_eq negb_and.
+  case Hbrc: ((block_round (qc_vote_data (qc_of c))) <= round c);
+    [rewrite orbF andbT andTb -ltnNge => Hcpc | rewrite andbF andTb => _ ].
+  - by rewrite ltnNge; move/ltnW: (leq_trans Hcpc Hcpb)=> Hbb; rewrite Hbb (leq_trans Hbrc Hbb) /=.
+  move/negbT: Hbrc; rewrite -ltnNge=> Hbrc; case Hqbb: (block_round (qc_vote_data (qc_of c)) <= round b); first by [].
+  move/negbT: Hqbb; rewrite -ltnNge=> Hqbb; rewrite maxnAC; rewrite  [maxn (round b).+1 _]maxnCA; move/maxn_idPr: (Hqbb)=>->.
+  rewrite 2!maxnA -/(comparator state) [maxn (maxn (comparator _) _) _]maxnAC; move/ltnW: (leq_ltn_trans Hcpb Hqbb); move/maxn_idPr=>->.
+  move: (leq_maxr (last_vote_round state).+1 (preferred_block_round state)); rewrite -/(comparator state)=> Hprcsb.
+  by rewrite maxnAC; move: (leq_ltn_trans (leq_trans Hprcsb Hcpb) Hqbb); move/ltnW/maxn_idPr=>->.
+by rewrite andbAC -voting_comparator_eq Hc andFb andbAC -voting_comparator_eq Hb andFb.
+Qed.
+
+Lemma comparator_next state1 state2 b:
+  comparator state1 = comparator state2
+  -> comparator (next_state state1 b) = comparator (next_state state2 b).
+Proof.
+move=> H12; case H1: (voted_on state1 b); move: (H1); rewrite voting_comparator_eq H12 -voting_comparator_eq=> H2.
+- by rewrite (voting_comparator H1) (voting_comparator H2).
+by rewrite (non_voting_comparator (negbT H1)) (non_voting_comparator (negbT H2)) H12.
+Qed.
+
+Lemma comparator_processing state1 state2 bseq:
+  comparator state1 = comparator state2
+  -> comparator (node_processing state1 bseq).1 = comparator (node_processing state2 bseq).1.
+Proof.
+elim: bseq state1 state2 =>[| x s IHs] state1 state2 H12 //.
+by rewrite 2!node_processing_cons1 (IHs _ _ (comparator_next x H12)).
+Qed.
+
+Lemma comparator_push_right state bs b:
+  comparator (node_processing state (b::bs)).1 = comparator (node_processing state (rcons bs b)).1.
+Proof.
+elim: bs state b => [|x s IHs] state b //=.
+rewrite -rcons_cons -node_processing_rcons; move/comparator_next: (IHs state x)=>->.
+rewrite -node_processing_rcons comparatorC 2!node_processing_rcons.
+rewrite node_processing_cons1 IHs -node_processing_cons1 -rcons_cons -node_processing_rcons.
+by move/comparator_next: (IHs state b)=>->; rewrite node_processing_rcons.
+Qed.
+
+Lemma next_state_repeat state b:
+  (next_state (next_state state b) b) = (next_state state b).
+Proof.
+rewrite next_state_lvr_if voting_next_N update_maxn next_state_pbr_update update_maxn  /= -maxnA maxnn.
+rewrite -/(preferred_block_round {| last_vote_round := last_vote_round state;
+  preferred_block_round := maxn (preferred_block_round state) (block_round (qc_vote_data (qc_of b))) |}).
+rewrite -update_maxn -next_state_pbr_update.
+have H: forall s, s = {| last_vote_round := (last_vote_round s);
+                    preferred_block_round:= (preferred_block_round s)|}; first by case.
+by rewrite {3}(H (next_state state b)).
+Qed.
+
+Lemma comparator_repeat state b:
+  comparator (next_state (next_state state b) b) =
+  comparator (next_state state b).
+Proof.
+by rewrite next_state_repeat.
+Qed.
+
+Lemma comparator_predC1 state bs b:
+  b \in bs ->
+  comparator (node_processing state bs).1 =
+  comparator (node_processing (next_state state b) (filter (predC1 b) bs)).1.
+Proof.
+elim: bs state b =>[|x s IHs] // state b.
+rewrite in_cons node_processing_cons1; case Hx: (b \in s).
+- move=>_; rewrite (IHs _ _ Hx); case Hbx: (b == x).
+  - by move/eqP: Hbx=>->; rewrite (comparator_processing _ (comparator_repeat _ _)) {2}/filter /predC1 /= eq_refl /=.
+   by rewrite (comparator_processing _ (comparatorC state x b)) {2}/filter /predC1 /= eq_sym Hbx /= -node_processing_cons1.
+rewrite orbF=> Hbx; move/negbT: Hx; rewrite -not_in_all_predC1; move/all_filterP; rewrite /filter /predC1 /= eq_sym Hbx /==>->.
+by move/eqP: Hbx=><-.
+Qed.
+
+Lemma comparator_orderfree state bs1 bs2:
+  bs1 =i bs2 ->
+  comparator (node_processing state bs1).1 = comparator (node_processing state bs2).1.
+Proof.
+elim: bs1 state bs2 => [|x s IHs] state bs2 H12 //; last rewrite node_processing_cons1.
+- by case: bs2 H12 => [|x2 s2] H12 //; move: (H12 x2); rewrite in_nil in_cons eq_refl.
+case Hx: (x \in s).
+- have: s=ibs2; first by move=> y; rewrite -H12 in_cons; move: Hx; case Hxy: (y == x); [move/eqP: Hxy=>->->| rewrite orFb].
+  move: (predC1_split Hx); move/IHs=>->; rewrite node_processing_cons1 (comparator_processing _ (comparator_repeat state x)).
+  rewrite -node_processing_cons1; move/IHs: (predC1_split Hx)=><-; apply IHs.
+have: s=i (filter (predC1 x) bs2); first move => y.
+- move: (H12 y); rewrite in_cons mem_filter /predC1 /=; case Hyx: (y == x); by [move/eqP: Hyx=>->| rewrite andTb orFb].
+  by move/IHs=>->; move: (mem_head x s); rewrite H12; move/comparator_predC1=>->.
+Qed.
+
+Lemma voted_in_processing_repeat state b bs:
+  voted_in_processing (next_state state b) (b:: bs) =
+  voted_in_processing (next_state state b) (bs).
+Proof.
+rewrite /voted_in_processing !node_processing_cons !mask_cons.
+by rewrite voting_next_N next_state_repeat.
+Qed.
+
+Lemma voted_in_processing_comparison state1 state2 bs:
+  comparator state1 = comparator state2 ->
+  voted_in_processing state1 bs = voted_in_processing state2 bs.
+Proof.
+elim: bs state1 state2=>[| x s IHs] state1 state2 H12 //.
+rewrite /voted_in_processing 2!node_processing_cons 2!mask_cons.
+rewrite -/(map snd) -/unzip2 -2!/(voted_in_processing (next_state _ x) s).
+rewrite (IHs _ _ (comparator_next x H12)) /=.
+by rewrite 2!voting_comparator_eq H12.
+Qed.
+
+Lemma voted_in_predC1 state b bs:
+  voted_in_processing (next_state state b) (bs) =
+  voted_in_processing (next_state state b) (filter (predC1 b) bs).
+Proof.
+elim: bs state b =>[| x s IHs] state b //=.
+case Hbx: (x == b)=>/=.
+- move/eqP: Hbx=>->; rewrite {1}/voted_in_processing node_processing_cons mask_cons.
+  rewrite next_state_repeat voting_next_N -/(map snd) -/unzip2.
+  by rewrite -/(voted_in_processing (next_state state b) s) IHs.
+rewrite /voted_in_processing 2![(node_processing _ (x:: _)).2]node_processing_cons.
+rewrite 2!mask_cons -/(map snd) -/unzip2 -/(voted_in_processing _ s).
+rewrite (voted_in_processing_comparison _ (comparatorC _ _ _)) IHs.
+by rewrite (voted_in_processing_comparison _ (comparatorC _ _ _)).
+Qed.
+
+Lemma voted_in_rundup state bs:
+  voted_in_processing state bs = voted_in_processing state (rundup bs).
+Proof.
+elim: bs state =>[| x s IHs] state //=.
+rewrite /voted_in_processing 2!node_processing_cons /unzip2 map_cons mask_cons.
+rewrite -/(voted_in_processing (next_state state x) s) IHs .
+rewrite mask_cons -/(map snd) -/unzip2 -/(voted_in_processing (next_state state x) _).
+by rewrite -voted_in_predC1.
+Qed.
+
+Lemma voted_in_processing_state_orderfree state bs1 bs2 bseq:
+  bs1 =i bs2 ->
+  voted_in_processing (node_processing state bs1).1 bseq =
+  voted_in_processing (node_processing state bs2).1 bseq.
+Proof.
+move=> H; apply (voted_in_processing_comparison _ (comparator_orderfree _ H)).
+Qed.
+
+Lemma voted_in_processing_idx state bseq b:
+  (b \in (voted_in_processing state bseq)) =
+  (voted_on (nth state (unzip1 (node_processing state bseq).2) (index b bseq) ) b && (b \in bseq)).
+Proof.
+rewrite voted_in_rundup.
+elim: bseq b state =>[| bb bbs IHbb] b state /=.
+- by rewrite in_nil andbF.
+rewrite /voted_in_processing /= 2!node_processing_cons /unzip2 mask_cons -/(map snd) /=.
+case H: (bb == b).
+- move/eqP: H=> ->; rewrite in_cons eqxx.
+  case H2: (voted_on state b); first by rewrite in_cons eqxx orTb andbT.
+  rewrite /=; apply: negbTE; apply: contraT; move/negPn=>H.
+  by move: (mem_mask H); rewrite mem_filter /= eq_refl.
+rewrite mem_cat mem_nseq in_cons eq_sym H andbF 2!orFb.
+rewrite -/unzip2 -/(voted_in_processing (next_state state bb) _).
+rewrite -voted_in_predC1 IHbb /=; case Hbbs: (b\in bbs); last by rewrite 2!andbF.
+rewrite (nth_in_default_irrel (next_state state bb) state _); first by [].
+by rewrite size_map size_processing index_mem.
+Qed.
+
+(************************************************************)
+(** Node Aggregation                                       **)
+(************************************************************)
+
+
+Definition node_aggregator bseq :=
+  (foldl (fun stateNvote => voting_rule stateNvote.1) (genesis_state,false) bseq).1.
+
+
+Definition commit_rule state (qc: QC)(bround: nat) :=
+  let: potential_commit_round := (parent_block_round (qc_vote_data qc)) in
+  if (potential_commit_round.+1 == (block_round (qc_vote_data qc))) &&
+        ((block_round (qc_vote_data qc)).+1 == bround) then
+    Some(potential_commit_round)
+  else None.
+
+End State.
